src/riot/RIoT.X509.AliasKeyCRT.fst
@@ -15,98 +15,98 @@ open LowParse.Spec.SeqBytes.Base
 open LowParse.Spec.Bytes
 
 #push-options "--z3rlimit 32"
-type aliasKeyCRT_t (tbs_len: asn1_int32) = {
+type aliasKeyCRT_payload_t (tbs_len: asn1_int32) = {
   aliasKeyCRT_tbs: B32.lbytes32 tbs_len;
-  aliasKeyCRT_sig_alg: algorithmIdentifier_t_inbound;
+  aliasKeyCRT_sig_alg: algorithmIdentifier_t;
   aliasKeyCRT_sig: x509_signature_t
 }
 #pop-options
 
-let aliasKeyCRT_t' (tbs_len: asn1_int32) = (
+let aliasKeyCRT_payload_t' (tbs_len: asn1_int32) = (
   (B32.lbytes32 tbs_len `tuple2`
-   algorithmIdentifier_t_inbound) `tuple2`
+   algorithmIdentifier_t) `tuple2`
    x509_signature_t
 )
 
-let synth_aliasKeyCRT_t
+let synth_aliasKeyCRT_payload_t
   (tbs_len: asn1_int32)
-  (x': aliasKeyCRT_t' tbs_len)
-: GTot (aliasKeyCRT_t tbs_len)
+  (x': aliasKeyCRT_payload_t' tbs_len)
+: GTot (aliasKeyCRT_payload_t tbs_len)
 = { aliasKeyCRT_tbs     = fst (fst x');
     aliasKeyCRT_sig_alg = snd (fst x');
     aliasKeyCRT_sig     = snd x' }
 
-let synth_aliasKeyCRT_t'
+let synth_aliasKeyCRT_payload_t'
   (tbs_len: asn1_int32)
-  (x: aliasKeyCRT_t tbs_len)
-: Tot (x': aliasKeyCRT_t' tbs_len { x == synth_aliasKeyCRT_t tbs_len x' })
+  (x: aliasKeyCRT_payload_t tbs_len)
+: Tot (x': aliasKeyCRT_payload_t' tbs_len { x == synth_aliasKeyCRT_payload_t tbs_len x' })
 = (x.aliasKeyCRT_tbs,
    x.aliasKeyCRT_sig_alg),
    x.aliasKeyCRT_sig
 
-let parse_aliasKeyCRT
+let parse_aliasKeyCRT_payload
   (tbs_len: asn1_int32)
-: parser _ (aliasKeyCRT_t tbs_len)
+: parser _ (aliasKeyCRT_payload_t tbs_len)
 = parse_flbytes32 tbs_len
   `nondep_then`
-  parse_algorithmIdentifier_sequence_TLV
+  parse_algorithmIdentifier
   `nondep_then`
   parse_x509_signature
   `parse_synth`
-  synth_aliasKeyCRT_t tbs_len
+  synth_aliasKeyCRT_payload_t tbs_len
 
-let serialize_aliasKeyCRT
+let serialize_aliasKeyCRT_payload
   (tbs_len: asn1_int32)
-: serializer (parse_aliasKeyCRT tbs_len)
+: serializer (parse_aliasKeyCRT_payload tbs_len)
 = serialize_synth
   (* p1 *) (parse_flbytes32 tbs_len
             `nondep_then`
-            parse_algorithmIdentifier_sequence_TLV
+            parse_algorithmIdentifier
             `nondep_then`
             parse_x509_signature)
-  (* f2 *) (synth_aliasKeyCRT_t tbs_len)
+  (* f2 *) (synth_aliasKeyCRT_payload_t tbs_len)
   (* s1 *) (serialize_flbytes32 tbs_len
             `serialize_nondep_then`
-            serialize_algorithmIdentifier_sequence_TLV
+            serialize_algorithmIdentifier
             `serialize_nondep_then`
             serialize_x509_signature)
-  (* g1 *) (synth_aliasKeyCRT_t' tbs_len)
+  (* g1 *) (synth_aliasKeyCRT_payload_t' tbs_len)
   (* prf*) ()
 
-let lemma_serialize_aliasKeyCRT_unfold
+let lemma_serialize_aliasKeyCRT_payload_unfold
   (tbs_len: asn1_int32)
-  (x: aliasKeyCRT_t tbs_len)
+  (x: aliasKeyCRT_payload_t tbs_len)
 : Lemma (
-  serialize_aliasKeyCRT tbs_len `serialize` x ==
+  serialize_aliasKeyCRT_payload tbs_len `serialize` x ==
  (serialize_flbytes32 tbs_len `serialize` x.aliasKeyCRT_tbs)
   `Seq.append`
- (serialize_algorithmIdentifier_sequence_TLV `serialize` x.aliasKeyCRT_sig_alg)
+ (serialize_algorithmIdentifier `serialize` x.aliasKeyCRT_sig_alg)
   `Seq.append`
  (serialize_x509_signature `serialize` x.aliasKeyCRT_sig)
 )
 = serialize_nondep_then_eq
   (* s1 *) (serialize_flbytes32 tbs_len)
-  (* s2 *) (serialize_algorithmIdentifier_sequence_TLV)
-  (* in *) (fst (synth_aliasKeyCRT_t' tbs_len x));
+  (* s2 *) (serialize_algorithmIdentifier)
+  (* in *) (fst (synth_aliasKeyCRT_payload_t' tbs_len x));
   serialize_nondep_then_eq
   (* s1 *) (serialize_flbytes32 tbs_len
             `serialize_nondep_then`
-            serialize_algorithmIdentifier_sequence_TLV)
+            serialize_algorithmIdentifier)
   (* s2 *) (serialize_x509_signature)
-  (* in *) (synth_aliasKeyCRT_t' tbs_len x);
+  (* in *) (synth_aliasKeyCRT_payload_t' tbs_len x);
   serialize_synth_eq
   (* p1 *) (parse_flbytes32 tbs_len
             `nondep_then`
-            parse_algorithmIdentifier_sequence_TLV
+            parse_algorithmIdentifier
             `nondep_then`
             parse_x509_signature)
-  (* f2 *) (synth_aliasKeyCRT_t tbs_len)
+  (* f2 *) (synth_aliasKeyCRT_payload_t tbs_len)
   (* s1 *) (serialize_flbytes32 tbs_len
             `serialize_nondep_then`
-            serialize_algorithmIdentifier_sequence_TLV
+            serialize_algorithmIdentifier
             `serialize_nondep_then`
             serialize_x509_signature)
-  (* g1 *) (synth_aliasKeyCRT_t' tbs_len)
+  (* g1 *) (synth_aliasKeyCRT_payload_t' tbs_len)
   (* prf*) ()
   (* in *) x
 
@@ -126,55 +126,56 @@ let len_of_aliasKeyCRT_payload
 
 #restart-solver
 #push-options "--z3rlimit 64 --fuel 0 --ifuel 0"
-let lemma_serialize_aliasKeyCRT_size
+let lemma_serialize_aliasKeyCRT_payload_size
   (tbs_len: asn1_int32)
-  (x: aliasKeyCRT_t tbs_len)
+  (x: aliasKeyCRT_payload_t tbs_len)
 : Lemma (
   (* unfold *)
-  length_of_opaque_serialization (serialize_aliasKeyCRT tbs_len) x ==
+  length_of_opaque_serialization (serialize_aliasKeyCRT_payload tbs_len) x ==
   length_of_opaque_serialization (serialize_flbytes32 tbs_len) x.aliasKeyCRT_tbs +
-  length_of_opaque_serialization (serialize_algorithmIdentifier_sequence_TLV) x.aliasKeyCRT_sig_alg +
+  length_of_opaque_serialization (serialize_algorithmIdentifier) x.aliasKeyCRT_sig_alg +
   length_of_opaque_serialization (serialize_x509_signature) x.aliasKeyCRT_sig /\
   (* exact size *)
-  length_of_opaque_serialization (serialize_aliasKeyCRT tbs_len) x
+  length_of_opaque_serialization (serialize_aliasKeyCRT_payload tbs_len) x
   == length_of_aliasKeyCRT_payload tbs_len
 )
-= lemma_serialize_aliasKeyCRT_unfold tbs_len x;
-  (**) lemma_serialize_algorithmIdentifier_sequence_TLV_size_exact x.aliasKeyCRT_sig_alg;
+= lemma_serialize_aliasKeyCRT_payload_unfold tbs_len x;
+  (**) lemma_serialize_algorithmIdentifier_size_exact x.aliasKeyCRT_sig_alg;
   (**) lemma_serialize_x509_signature_size      x.aliasKeyCRT_sig
 #pop-options
 
+
 (* SEQUENCE TLV*)
-let aliasKeyCRT_t_inbound
+let aliasKeyCRT_t
   (tbs_len: asn1_int32)
-= inbound_sequence_value_of (serialize_aliasKeyCRT tbs_len)
+= inbound_sequence_value_of (serialize_aliasKeyCRT_payload tbs_len)
 
-let parse_aliasKeyCRT_sequence_TLV
+let parse_aliasKeyCRT
   (tbs_len: asn1_int32)
-: parser (parse_asn1_envelop_tag_with_TLV_kind SEQUENCE) (aliasKeyCRT_t_inbound tbs_len)
-= aliasKeyCRT_t_inbound tbs_len
+: parser (parse_asn1_envelop_tag_with_TLV_kind SEQUENCE) (aliasKeyCRT_t tbs_len)
+= aliasKeyCRT_t tbs_len
   `coerce_parser`
-  parse_asn1_sequence_TLV (serialize_aliasKeyCRT tbs_len)
+  parse_asn1_sequence_TLV (serialize_aliasKeyCRT_payload tbs_len)
 
-let serialize_aliasKeyCRT_sequence_TLV
+let serialize_aliasKeyCRT
   (tbs_len: asn1_int32)
-: serializer (parse_aliasKeyCRT_sequence_TLV tbs_len)
+: serializer (parse_aliasKeyCRT tbs_len)
 = coerce_parser_serializer
-    (parse_aliasKeyCRT_sequence_TLV tbs_len)
-    (serialize_asn1_sequence_TLV (serialize_aliasKeyCRT tbs_len))
+    (parse_aliasKeyCRT tbs_len)
+    (serialize_asn1_sequence_TLV (serialize_aliasKeyCRT_payload tbs_len))
     ()
 
-let lemma_serialize_aliasKeyCRT_sequence_TLV_unfold
+let lemma_serialize_aliasKeyCRT_unfold
   (tbs_len: asn1_int32)
-  (x: aliasKeyCRT_t_inbound tbs_len)
-: Lemma ( predicate_serialize_asn1_sequence_TLV_unfold (serialize_aliasKeyCRT tbs_len) x )
-= lemma_serialize_asn1_sequence_TLV_unfold (serialize_aliasKeyCRT tbs_len) x
+  (x: aliasKeyCRT_t tbs_len)
+: Lemma ( predicate_serialize_asn1_sequence_TLV_unfold (serialize_aliasKeyCRT_payload tbs_len) x )
+= lemma_serialize_asn1_sequence_TLV_unfold (serialize_aliasKeyCRT_payload tbs_len) x
 
-let lemma_serialize_aliasKeyCRT_sequence_TLV_size
+let lemma_serialize_aliasKeyCRT_size
   (tbs_len: asn1_int32)
-  (x: aliasKeyCRT_t_inbound tbs_len)
-: Lemma ( predicate_serialize_asn1_sequence_TLV_size (serialize_aliasKeyCRT tbs_len) x )
-= lemma_serialize_asn1_sequence_TLV_size (serialize_aliasKeyCRT tbs_len) x
+  (x: aliasKeyCRT_t tbs_len)
+: Lemma ( predicate_serialize_asn1_sequence_TLV_size (serialize_aliasKeyCRT_payload tbs_len) x )
+= lemma_serialize_asn1_sequence_TLV_size (serialize_aliasKeyCRT_payload tbs_len) x
 
 let length_of_aliasKeyCRT
   (tbs_len: asn1_int32
@@ -195,70 +196,70 @@ let len_of_aliasKeyCRT
 #pop-options
 
 #push-options "--z3rlimit 64 --fuel 0 --ifuel 0"
-let lemma_serialize_aliasKeyCRT_sequence_TLV_size_exact
+let lemma_serialize_aliasKeyCRT_size_exact
   (tbs_len: asn1_int32)
-  (x: aliasKeyCRT_t_inbound tbs_len)
+  (x: aliasKeyCRT_t tbs_len)
 : Lemma (
-  let _ = lemma_serialize_aliasKeyCRT_size tbs_len x in
+  let _ = lemma_serialize_aliasKeyCRT_payload_size tbs_len x in
   (* exact size *)
-  length_of_opaque_serialization (serialize_aliasKeyCRT_sequence_TLV tbs_len) x
+  length_of_opaque_serialization (serialize_aliasKeyCRT tbs_len) x
   == length_of_aliasKeyCRT tbs_len /\
   (* upper bound *)
-  length_of_opaque_serialization (serialize_aliasKeyCRT_sequence_TLV tbs_len) x
+  length_of_opaque_serialization (serialize_aliasKeyCRT tbs_len) x
   <= v tbs_len + 84
 )
-= lemma_serialize_aliasKeyCRT_sequence_TLV_size tbs_len x;
-  (**) lemma_serialize_aliasKeyCRT_size tbs_len x
+= lemma_serialize_aliasKeyCRT_size tbs_len x;
+  (**) lemma_serialize_aliasKeyCRT_payload_size tbs_len x
 #pop-options
 
 
 (* low *)
 
-let serialize32_aliasKeyCRT_backwards
+let serialize32_aliasKeyCRT_payload_backwards
   (tbs_len: asn1_int32)
-: serializer32_backwards (serialize_aliasKeyCRT tbs_len)
+: serializer32_backwards (serialize_aliasKeyCRT_payload tbs_len)
 = serialize32_synth_backwards
   (* s1 *) (serialize32_flbytes32_backwards tbs_len
             `serialize32_nondep_then_backwards`
-            serialize32_algorithmIdentifier_sequence_TLV_backwards
+            serialize32_algorithmIdentifier_backwards
             `serialize32_nondep_then_backwards`
             serialize32_x509_signature_backwards)
-  (* f2 *) (synth_aliasKeyCRT_t  tbs_len)
-  (* g1 *) (synth_aliasKeyCRT_t' tbs_len)
-  (* g1'*) (synth_aliasKeyCRT_t' tbs_len)
+  (* f2 *) (synth_aliasKeyCRT_payload_t  tbs_len)
+  (* g1 *) (synth_aliasKeyCRT_payload_t' tbs_len)
+  (* g1'*) (synth_aliasKeyCRT_payload_t' tbs_len)
   (* prf*) ()
 
-let serialize32_aliasKeyCRT_sequence_TLV_backwards
+let serialize32_aliasKeyCRT_backwards
   (tbs_len: asn1_int32)
-: serializer32_backwards (serialize_aliasKeyCRT_sequence_TLV tbs_len)
+: serializer32_backwards (serialize_aliasKeyCRT tbs_len)
 = coerce_serializer32_backwards
-    (serialize_aliasKeyCRT_sequence_TLV tbs_len)
+    (serialize_aliasKeyCRT tbs_len)
     (serialize32_asn1_sequence_TLV_backwards
-       (serialize32_aliasKeyCRT_backwards tbs_len))
+       (serialize32_aliasKeyCRT_payload_backwards tbs_len))
     ()
 
 #restart-solver
 #push-options "--z3rlimit 32 --fuel 0 --ifuel 0"
 let x509_get_AliasKeyCRT
   (tbs_len: asn1_int32
-            { v tbs_len + 76 <= asn1_value_length_max_of_type SEQUENCE })
+            { length_of_aliasKeyCRT_payload tbs_len <= asn1_value_length_max_of_type SEQUENCE })
   (aliasKeyCRT_tbs: B32.lbytes32 tbs_len)
   (signature32: x509_signature_raw_t) // B32.lbytes32 64ul
-: Tot (aliasKeyCRT_t_inbound tbs_len)
+: Tot (aliasKeyCRT_t tbs_len)
 =
   let aliasKeyCRT_sig_alg = x509_get_algorithmIdentifier () in
-  (* Prf *) lemma_serialize_algorithmIdentifier_sequence_TLV_size_exact aliasKeyCRT_sig_alg;
+  (* Prf *) lemma_serialize_algorithmIdentifier_size_exact aliasKeyCRT_sig_alg;
 
   let aliasKeyCRT_sig = x509_get_signature signature32 in
   (* Prf *) lemma_serialize_x509_signature_size aliasKeyCRT_sig;
 
-  let aliasKeyCRT: aliasKeyCRT_t tbs_len = {
+  let aliasKeyCRT: aliasKeyCRT_payload_t tbs_len = {
     aliasKeyCRT_tbs     = aliasKeyCRT_tbs;
     aliasKeyCRT_sig_alg = aliasKeyCRT_sig_alg;
     aliasKeyCRT_sig     = aliasKeyCRT_sig
   } in
-  (* Prf *) lemma_serialize_aliasKeyCRT_unfold tbs_len aliasKeyCRT;
-  (* Prf *) lemma_serialize_aliasKeyCRT_size   tbs_len aliasKeyCRT;
+  (* Prf *) lemma_serialize_aliasKeyCRT_payload_unfold tbs_len aliasKeyCRT;
+  (* Prf *) lemma_serialize_aliasKeyCRT_payload_size   tbs_len aliasKeyCRT;
   (* Prf *) (**) lemma_serialize_flbytes32_size tbs_len aliasKeyCRT.aliasKeyCRT_tbs;
 
 (* return *) aliasKeyCRT
