src/riot/RIoT.X509.AliasKeyTBS.fst
@@ -15,7 +15,7 @@ module B32 = FStar.Bytes
 open LowParse.Spec.SeqBytes.Base
 open LowParse.Spec.Bytes
 
-type aliasKeyTBS_t (header_len: asn1_int32) = {
+type aliasKeyTBS_payload_t (header_len: asn1_int32) = {
 (* TEMPLATE of
  *       version         [0]  EXPLICIT Version DEFAULT v1,
  *       serialNumber         CertificateSerialNumber,
@@ -28,99 +28,99 @@ type aliasKeyTBS_t (header_len: asn1_int32) = {
  (*
   *      subjectPublicKeyInfo SubjectPublicKeyInfo
   *)
-  aliasKeyTBS_aliasKey_pub: subjectPublicKeyInfo_t_inbound;
+  aliasKeyTBS_aliasKey_pub: subjectPublicKeyInfo_t;
  (*
   *      extensions      [3]  EXPLICIT Extensions OPTIONAL
   *)
   aliasKeyTBS_extensions  : x509_extensions_t_inbound
-                              serialize_aliasKeyTBS_extensions_sequence_TLV
+                              serialize_aliasKeyTBS_extensions
 }
 
-let aliasKeyTBS_t' (header_len: asn1_int32) = (
+let aliasKeyTBS_payload_t' (header_len: asn1_int32) = (
    B32.lbytes32 header_len `tuple2`
-   subjectPublicKeyInfo_t_inbound `tuple2`
-   x509_extensions_t_inbound serialize_aliasKeyTBS_extensions_sequence_TLV
+   subjectPublicKeyInfo_t `tuple2`
+   x509_extensions_t_inbound serialize_aliasKeyTBS_extensions
 )
 
-let synth_aliasKeyTBS_t
+let synth_aliasKeyTBS_payload_t
   (header_len: asn1_int32)
-  (x': aliasKeyTBS_t' header_len)
-: GTot (aliasKeyTBS_t header_len)
+  (x': aliasKeyTBS_payload_t' header_len)
+: GTot (aliasKeyTBS_payload_t header_len)
 = { aliasKeyTBS_template     = fst (fst x');
     aliasKeyTBS_aliasKey_pub = snd (fst x');
     aliasKeyTBS_extensions   = snd x' }
 
-let synth_aliasKeyTBS_t'
+let synth_aliasKeyTBS_payload_t'
   (header_len: asn1_int32)
-  (x: aliasKeyTBS_t header_len)
-: Tot (x': aliasKeyTBS_t' header_len { x == synth_aliasKeyTBS_t header_len x' })
+  (x: aliasKeyTBS_payload_t header_len)
+: Tot (x': aliasKeyTBS_payload_t' header_len { x == synth_aliasKeyTBS_payload_t header_len x' })
 = (x.aliasKeyTBS_template,
    x.aliasKeyTBS_aliasKey_pub),
    x.aliasKeyTBS_extensions
 
-let parse_aliasKeyTBS
+let parse_aliasKeyTBS_payload
   (header_len: asn1_int32)
-: parser _ (aliasKeyTBS_t header_len)
+: parser _ (aliasKeyTBS_payload_t header_len)
 = parse_flbytes32 header_len
   `nondep_then`
-  parse_subjectPublicKeyInfo_sequence_TLV
+  parse_subjectPublicKeyInfo
   `nondep_then`
-  parse_x509_extensions_TLV serialize_aliasKeyTBS_extensions_sequence_TLV
+  parse_x509_extensions_TLV serialize_aliasKeyTBS_extensions
   `parse_synth`
-  synth_aliasKeyTBS_t header_len
+  synth_aliasKeyTBS_payload_t header_len
 
-let serialize_aliasKeyTBS
+let serialize_aliasKeyTBS_payload
   (header_len: asn1_int32)
-: serializer (parse_aliasKeyTBS header_len)
+: serializer (parse_aliasKeyTBS_payload header_len)
 = serialize_synth
   (* p1 *) (parse_flbytes32 header_len
             `nondep_then`
-            parse_subjectPublicKeyInfo_sequence_TLV
+            parse_subjectPublicKeyInfo
             `nondep_then`
-            parse_x509_extensions_TLV serialize_aliasKeyTBS_extensions_sequence_TLV)
-  (* f2 *) (synth_aliasKeyTBS_t header_len)
+            parse_x509_extensions_TLV serialize_aliasKeyTBS_extensions)
+  (* f2 *) (synth_aliasKeyTBS_payload_t header_len)
   (* s1 *) (serialize_flbytes32 header_len
             `serialize_nondep_then`
-            serialize_subjectPublicKeyInfo_sequence_TLV
+            serialize_subjectPublicKeyInfo
             `serialize_nondep_then`
-            serialize_x509_extensions_TLV serialize_aliasKeyTBS_extensions_sequence_TLV)
-  (* g1 *) (synth_aliasKeyTBS_t' header_len)
+            serialize_x509_extensions_TLV serialize_aliasKeyTBS_extensions)
+  (* g1 *) (synth_aliasKeyTBS_payload_t' header_len)
   (* prf*) ()
 
-let lemma_serialize_aliasKeyTBS_unfold
+let lemma_serialize_aliasKeyTBS_payload_unfold
   (header_len: asn1_int32)
-  (x: aliasKeyTBS_t header_len)
+  (x: aliasKeyTBS_payload_t header_len)
 : Lemma (
-  serialize_aliasKeyTBS header_len `serialize` x ==
+  serialize_aliasKeyTBS_payload header_len `serialize` x ==
  (serialize_flbytes32 header_len `serialize` x.aliasKeyTBS_template)
   `Seq.append`
- (serialize_subjectPublicKeyInfo_sequence_TLV `serialize` x.aliasKeyTBS_aliasKey_pub)
+ (serialize_subjectPublicKeyInfo `serialize` x.aliasKeyTBS_aliasKey_pub)
   `Seq.append`
- (serialize_x509_extensions_TLV serialize_aliasKeyTBS_extensions_sequence_TLV `serialize` x.aliasKeyTBS_extensions)
+ (serialize_x509_extensions_TLV serialize_aliasKeyTBS_extensions `serialize` x.aliasKeyTBS_extensions)
 )
 = serialize_nondep_then_eq
   (* s1 *) (serialize_flbytes32 header_len)
-  (* s2 *) (serialize_subjectPublicKeyInfo_sequence_TLV)
-  (* in *) (fst (synth_aliasKeyTBS_t' header_len x));
+  (* s2 *) (serialize_subjectPublicKeyInfo)
+  (* in *) (fst (synth_aliasKeyTBS_payload_t' header_len x));
   serialize_nondep_then_eq
   (* s1 *) (serialize_flbytes32 header_len
             `serialize_nondep_then`
-            serialize_subjectPublicKeyInfo_sequence_TLV)
-  (* s2 *) (serialize_x509_extensions_TLV serialize_aliasKeyTBS_extensions_sequence_TLV)
-  (* in *) (synth_aliasKeyTBS_t' header_len x);
+            serialize_subjectPublicKeyInfo)
+  (* s2 *) (serialize_x509_extensions_TLV serialize_aliasKeyTBS_extensions)
+  (* in *) (synth_aliasKeyTBS_payload_t' header_len x);
   serialize_synth_eq
   (* p1 *) (parse_flbytes32 header_len
             `nondep_then`
-            parse_subjectPublicKeyInfo_sequence_TLV
+            parse_subjectPublicKeyInfo
             `nondep_then`
-            parse_x509_extensions_TLV serialize_aliasKeyTBS_extensions_sequence_TLV)
-  (* f2 *) (synth_aliasKeyTBS_t header_len)
+            parse_x509_extensions_TLV serialize_aliasKeyTBS_extensions)
+  (* f2 *) (synth_aliasKeyTBS_payload_t header_len)
   (* s1 *) (serialize_flbytes32 header_len
             `serialize_nondep_then`
-            serialize_subjectPublicKeyInfo_sequence_TLV
+            serialize_subjectPublicKeyInfo
             `serialize_nondep_then`
-            serialize_x509_extensions_TLV serialize_aliasKeyTBS_extensions_sequence_TLV)
-  (* g1 *) (synth_aliasKeyTBS_t' header_len)
+            serialize_x509_extensions_TLV serialize_aliasKeyTBS_extensions)
+  (* g1 *) (synth_aliasKeyTBS_payload_t' header_len)
   (* prf*) ()
   (* in *) x
 
@@ -128,7 +128,7 @@ let lemma_serialize_aliasKeyTBS_unfold
 #push-options "--z3rlimit 64 --fuel 0 --ifuel 0"
 let length_of_aliasKeyTBS_payload
   (header_len: asn1_int32)
-  (ku: key_usage_t)
+  (ku: key_usage_payload_t)
   (version: datatype_of_asn1_type INTEGER)
 : GTot (nat)
 = v header_len +
@@ -137,7 +137,7 @@ let length_of_aliasKeyTBS_payload
 
 let len_of_aliasKeyTBS_payload
   (header_len: asn1_int32)
-  (ku: key_usage_t)
+  (ku: key_usage_payload_t)
   (version: datatype_of_asn1_type INTEGER
             { length_of_aliasKeyTBS_payload header_len ku version
               <= asn1_value_length_max_of_type SEQUENCE })
@@ -147,72 +147,72 @@ let len_of_aliasKeyTBS_payload
   len_of_subjectPublicKeyInfo +
   len_of_x509_extensions (len_of_aliasKeyTBS_extensions ku version)
 
-let lemma_serialize_aliasKeyTBS_size
+let lemma_serialize_aliasKeyTBS_payload_size
   (header_len: asn1_int32)
-  (x: aliasKeyTBS_t header_len)
+  (x: aliasKeyTBS_payload_t header_len)
 : Lemma (
   let riot_version = RIoT.X509.Extension.(x.aliasKeyTBS_extensions.aliasKeyTBS_extensions_riot.x509_extValue_riot.riot_version) in
   let ku = (snd x.aliasKeyTBS_extensions.aliasKeyTBS_extensions_key_usage) in
   (* unfold *)
-  length_of_opaque_serialization (serialize_aliasKeyTBS header_len)              x ==
+  length_of_opaque_serialization (serialize_aliasKeyTBS_payload header_len)              x ==
   length_of_opaque_serialization (serialize_flbytes32 header_len)                x.aliasKeyTBS_template     +
-  length_of_opaque_serialization (serialize_subjectPublicKeyInfo_sequence_TLV)   x.aliasKeyTBS_aliasKey_pub +
+  length_of_opaque_serialization (serialize_subjectPublicKeyInfo)   x.aliasKeyTBS_aliasKey_pub +
   length_of_opaque_serialization (serialize_x509_extensions_TLV
-                                  serialize_aliasKeyTBS_extensions_sequence_TLV) x.aliasKeyTBS_extensions /\
+                                  serialize_aliasKeyTBS_extensions) x.aliasKeyTBS_extensions /\
   (* exact size *)
-  length_of_opaque_serialization (serialize_aliasKeyTBS header_len)            x
+  length_of_opaque_serialization (serialize_aliasKeyTBS_payload header_len)            x
   == length_of_aliasKeyTBS_payload header_len ku riot_version
   (* upper bound *)
   // length_of_opaque_serialization (serialize_aliasKeyTBS header_len)            x
   // <= v header_len + 44 + (6 + (6 + 117))
 )
-= lemma_serialize_aliasKeyTBS_unfold header_len x;
+= lemma_serialize_aliasKeyTBS_payload_unfold header_len x;
     (* + v header_len *)
     (* + 44 *)
-    lemma_serialize_subjectPublicKeyInfo_sequence_TLV_size_exact x.aliasKeyTBS_aliasKey_pub;
+    lemma_serialize_subjectPublicKeyInfo_size_exact x.aliasKeyTBS_aliasKey_pub;
     (* + (6) *)
-    lemma_serialize_x509_extensions_TLV_size serialize_aliasKeyTBS_extensions_sequence_TLV x.aliasKeyTBS_extensions;
+    lemma_serialize_x509_extensions_TLV_size serialize_aliasKeyTBS_extensions x.aliasKeyTBS_extensions;
       (* + (6 + 117) / + |riot_veriosn| + 113 *)
-      lemma_serialize_aliasKeyTBS_extensions_sequence_TLV_size_exact x.aliasKeyTBS_extensions
+      lemma_serialize_aliasKeyTBS_extensions_size_exact x.aliasKeyTBS_extensions
 #pop-options
 
-// unfold
-let aliasKeyTBS_t_inbound
-  (header_len: asn1_int32)
-= inbound_sequence_value_of (serialize_aliasKeyTBS header_len)
 
-let parse_aliasKeyTBS_sequence_TLV
+let aliasKeyTBS_t
   (header_len: asn1_int32)
-: parser (parse_asn1_envelop_tag_with_TLV_kind SEQUENCE) (aliasKeyTBS_t_inbound header_len)
+= inbound_sequence_value_of (serialize_aliasKeyTBS_payload header_len)
+
+let parse_aliasKeyTBS
+  (header_len: asn1_int32)
+: parser (parse_asn1_envelop_tag_with_TLV_kind SEQUENCE) (aliasKeyTBS_t header_len)
 =
-  aliasKeyTBS_t_inbound header_len
+  aliasKeyTBS_t header_len
   `coerce_parser`
-  parse_asn1_sequence_TLV (serialize_aliasKeyTBS header_len)
+  parse_asn1_sequence_TLV (serialize_aliasKeyTBS_payload header_len)
 
-let serialize_aliasKeyTBS_sequence_TLV
+let serialize_aliasKeyTBS
   (header_len: asn1_int32)
-: serializer (parse_aliasKeyTBS_sequence_TLV header_len)
+: serializer (parse_aliasKeyTBS header_len)
 = coerce_parser_serializer
-    (parse_aliasKeyTBS_sequence_TLV header_len)
-    (serialize_asn1_sequence_TLV (serialize_aliasKeyTBS header_len))
+    (parse_aliasKeyTBS header_len)
+    (serialize_asn1_sequence_TLV (serialize_aliasKeyTBS_payload header_len))
     ()
 
-let lemma_serialize_aliasKeyTBS_sequence_TLV_unfold
+let lemma_serialize_aliasKeyTBS_unfold
   (header_len: asn1_int32)
-  (x: aliasKeyTBS_t_inbound header_len)
-: Lemma ( predicate_serialize_asn1_sequence_TLV_unfold (serialize_aliasKeyTBS header_len) x )
-= lemma_serialize_asn1_sequence_TLV_unfold (serialize_aliasKeyTBS header_len) x
+  (x: aliasKeyTBS_t header_len)
+: Lemma ( predicate_serialize_asn1_sequence_TLV_unfold (serialize_aliasKeyTBS_payload header_len) x )
+= lemma_serialize_asn1_sequence_TLV_unfold (serialize_aliasKeyTBS_payload header_len) x
 
-let lemma_serialize_aliasKeyTBS_sequence_TLV_size
+let lemma_serialize_aliasKeyTBS_size
   (header_len: asn1_int32)
-  (x: aliasKeyTBS_t_inbound header_len)
-: Lemma ( predicate_serialize_asn1_sequence_TLV_size (serialize_aliasKeyTBS header_len) x )
-= lemma_serialize_asn1_sequence_TLV_size (serialize_aliasKeyTBS header_len) x
+  (x: aliasKeyTBS_t header_len)
+: Lemma ( predicate_serialize_asn1_sequence_TLV_size (serialize_aliasKeyTBS_payload header_len) x )
+= lemma_serialize_asn1_sequence_TLV_size (serialize_aliasKeyTBS_payload header_len) x
 
 #push-options "--z3rlimit 64 --fuel 0 --ifuel 0"
 let length_of_aliasKeyTBS
   (header_len: asn1_int32)
-  (ku: key_usage_t)
+  (ku: key_usage_payload_t)
   (version: datatype_of_asn1_type INTEGER
             { length_of_aliasKeyTBS_payload header_len ku version
               <= asn1_value_length_max_of_type SEQUENCE })
@@ -221,7 +221,7 @@ let length_of_aliasKeyTBS
 
 let len_of_aliasKeyTBS
   (header_len: asn1_int32)
-  (ku: key_usage_t)
+  (ku: key_usage_payload_t)
   (version: datatype_of_asn1_type INTEGER
             { length_of_aliasKeyTBS_payload header_len ku version
               <= asn1_value_length_max_of_type SEQUENCE })
@@ -232,47 +232,47 @@ let len_of_aliasKeyTBS
 
 #restart-solver
 #push-options "--z3rlimit 64 --fuel 0 --ifuel 0"
-let lemma_serialize_aliasKeyTBS_sequence_TLV_size_exact
+let lemma_serialize_aliasKeyTBS_size_exact
   (header_len: asn1_int32)
-  (x: aliasKeyTBS_t_inbound header_len)
+  (x: aliasKeyTBS_t header_len)
 : Lemma (
   let riot_version = RIoT.X509.Extension.(x.aliasKeyTBS_extensions.aliasKeyTBS_extensions_riot.x509_extValue_riot.riot_version) in
   let ku = (snd x.aliasKeyTBS_extensions.aliasKeyTBS_extensions_key_usage) in
-  let _ = lemma_serialize_aliasKeyTBS_size header_len x in
+  let _ = lemma_serialize_aliasKeyTBS_payload_size header_len x in
   (* exact size *)
-  length_of_opaque_serialization (serialize_aliasKeyTBS_sequence_TLV header_len) x
+  length_of_opaque_serialization (serialize_aliasKeyTBS header_len) x
   == length_of_aliasKeyTBS header_len ku riot_version
   (* upper bound *)
-  // length_of_opaque_serialization (serialize_aliasKeyTBS_sequence_TLV header_len) x
+  // length_of_opaque_serialization (serialize_aliasKeyTBS header_len) x
   // <= (6 + v header_len + 44 + (6 + (6 + 117)))
 )
-= lemma_serialize_aliasKeyTBS_sequence_TLV_size header_len x;
-    lemma_serialize_aliasKeyTBS_size header_len x
+= lemma_serialize_aliasKeyTBS_size header_len x;
+    lemma_serialize_aliasKeyTBS_payload_size header_len x
 #pop-options
 
 
 (* low *)
-let serialize32_aliasKeyTBS_backwards
+let serialize32_aliasKeyTBS_payload_backwards
   (header_len: asn1_int32)
-: serializer32_backwards (serialize_aliasKeyTBS header_len)
+: serializer32_backwards (serialize_aliasKeyTBS_payload header_len)
 = serialize32_synth_backwards
   (* s1 *) (serialize32_flbytes32_backwards header_len
             `serialize32_nondep_then_backwards`
-            serialize32_subjectPublicKeyInfo_sequence_TLV_backwards
+            serialize32_subjectPublicKeyInfo_backwards
             `serialize32_nondep_then_backwards`
-            serialize32_x509_extensions_TLV_backwards serialize32_aliasKeyTBS_extensions_sequence_TLV_backwards)
-  (* f2 *) (synth_aliasKeyTBS_t  header_len)
-  (* g1 *) (synth_aliasKeyTBS_t' header_len)
-  (* g1'*) (synth_aliasKeyTBS_t' header_len)
+            serialize32_x509_extensions_TLV_backwards serialize32_aliasKeyTBS_extensions_backwards)
+  (* f2 *) (synth_aliasKeyTBS_payload_t  header_len)
+  (* g1 *) (synth_aliasKeyTBS_payload_t' header_len)
+  (* g1'*) (synth_aliasKeyTBS_payload_t' header_len)
   (* prf*) ()
 
-let serialize32_aliasKeyTBS_sequence_TLV_backwards
+let serialize32_aliasKeyTBS_backwards
   (header_len: asn1_int32)
-: serializer32_backwards (serialize_aliasKeyTBS_sequence_TLV header_len)
+: serializer32_backwards (serialize_aliasKeyTBS header_len)
 = coerce_serializer32_backwards
-  (* s2 *) (serialize_aliasKeyTBS_sequence_TLV header_len)
+  (* s2 *) (serialize_aliasKeyTBS header_len)
   (* s32*) (serialize32_asn1_sequence_TLV_backwards
-             (serialize32_aliasKeyTBS_backwards header_len))
+             (serialize32_aliasKeyTBS_payload_backwards header_len))
   (* prf*) ()
 
 
@@ -282,33 +282,33 @@ let serialize32_aliasKeyTBS_sequence_TLV_backwards
 let x509_get_AliasKeyTBS
   (header_len: asn1_int32)
   (aliasKeyTBS_template: B32.lbytes32 header_len)
-  (ku: key_usage_t)
+  (ku: key_usage_payload_t)
   (version: datatype_of_asn1_type INTEGER
             { length_of_aliasKeyTBS_payload header_len ku version
               <= asn1_value_length_max_of_type SEQUENCE })
   (fwid: B32.lbytes32 32ul)
   (deviceIDPub: B32.lbytes32 32ul)
   (aliasKeyPub: B32.lbytes32 32ul)
-: Tot (aliasKeyTBS_t_inbound header_len)
+: Tot (aliasKeyTBS_t header_len)
 =
   let aliasKeyTBS_extensions = x509_get_aliasKeyTBS_extensions
                                  ku
                                  version
                                  fwid
                                  deviceIDPub in
-  (* Prf *) lemma_serialize_aliasKeyTBS_extensions_sequence_TLV_size_exact aliasKeyTBS_extensions;
+  (* Prf *) lemma_serialize_aliasKeyTBS_extensions_size_exact aliasKeyTBS_extensions;
 
   let aliasKeyPubInfo = x509_get_subjectPublicKeyInfo
                            aliasKeyPub in
-  (* Prf *) lemma_serialize_subjectPublicKeyInfo_sequence_TLV_size_exact aliasKeyPubInfo;
+  (* Prf *) lemma_serialize_subjectPublicKeyInfo_size_exact aliasKeyPubInfo;
 
-  let aliasKeyTBS: aliasKeyTBS_t header_len = {
+  let aliasKeyTBS: aliasKeyTBS_payload_t header_len = {
     aliasKeyTBS_template       = aliasKeyTBS_template;
     aliasKeyTBS_aliasKey_pub   = aliasKeyPubInfo;
     aliasKeyTBS_extensions     = aliasKeyTBS_extensions
   } in
-  (* Prf *) lemma_serialize_aliasKeyTBS_unfold header_len aliasKeyTBS;
-  (* Prf *) lemma_serialize_aliasKeyTBS_size   header_len aliasKeyTBS;
+  (* Prf *) lemma_serialize_aliasKeyTBS_payload_unfold header_len aliasKeyTBS;
+  (* Prf *) lemma_serialize_aliasKeyTBS_payload_size   header_len aliasKeyTBS;
   (* Prf *) (**) lemma_serialize_flbytes32_size header_len aliasKeyTBS.aliasKeyTBS_template;
 
 (*return*) aliasKeyTBS
