src/riot/RIoT.X509.CompositeDeviceID.fst
@@ -12,194 +12,174 @@ open X509.Crypto
 open RIoT.X509.Base
 open RIoT.X509.FWID
 
-#set-options "--z3rlimit 32"
+#set-options "--z3rlimit 32 --fuel 0 --ifuel 0"
 
 (* CompositeDeviceID *)
-type compositeDeviceID_t
+type compositeDeviceID_payload_t
 = { riot_version : datatype_of_asn1_type INTEGER;
-    riot_deviceID: subjectPublicKeyInfo_t_inbound;
-    riot_fwid    : fwid_t_inbound }
+    riot_deviceID: subjectPublicKeyInfo_t;
+    riot_fwid    : fwid_t }
 
-let compositeDeviceID_t'
+let compositeDeviceID_payload_t'
 = ((datatype_of_asn1_type INTEGER &
-    subjectPublicKeyInfo_t_inbound) &
-    fwid_t_inbound)
+    subjectPublicKeyInfo_t) &
+    fwid_t)
 
 (* Serialier spec *)
-let synth_compositeDeviceID_t
-  (x': compositeDeviceID_t')
-: GTot (compositeDeviceID_t)
+let synth_compositeDeviceID_payload_t
+  (x': compositeDeviceID_payload_t')
+: GTot (compositeDeviceID_payload_t)
 = { riot_version  = fst (fst x');
     riot_deviceID = snd (fst x');
     riot_fwid     = snd x' }
 
-let synth_compositeDeviceID_t'
-  (x: compositeDeviceID_t)
-: Tot (x': compositeDeviceID_t' { x == synth_compositeDeviceID_t x' })
+let synth_compositeDeviceID_payload_t'
+  (x: compositeDeviceID_payload_t)
+: Tot (x': compositeDeviceID_payload_t' { x == synth_compositeDeviceID_payload_t x' })
 = ((x.riot_version, x.riot_deviceID), x.riot_fwid)
 
-let parse_compositeDeviceID
-: parser _ (compositeDeviceID_t)
+let parse_compositeDeviceID_payload
+: parser _ (compositeDeviceID_payload_t)
 = parse_asn1_TLV_of_type INTEGER
   `nondep_then`
-  parse_subjectPublicKeyInfo_sequence_TLV
+  parse_subjectPublicKeyInfo
   `nondep_then`
-  parse_fwid_sequence_TLV
+  parse_fwid
   `parse_synth`
-  synth_compositeDeviceID_t
+  synth_compositeDeviceID_payload_t
 
-let serialize_compositeDeviceID
-: serializer (parse_compositeDeviceID)
+let serialize_compositeDeviceID_payload
+: serializer (parse_compositeDeviceID_payload)
 = serialize_synth
   (* p1 *) (parse_asn1_TLV_of_type INTEGER
             `nondep_then`
-            parse_subjectPublicKeyInfo_sequence_TLV
+            parse_subjectPublicKeyInfo
             `nondep_then`
-            parse_fwid_sequence_TLV)
-  (* f2 *) (synth_compositeDeviceID_t)
+            parse_fwid)
+  (* f2 *) (synth_compositeDeviceID_payload_t)
   (* s1 *) (serialize_asn1_TLV_of_type INTEGER
             `serialize_nondep_then`
-            serialize_subjectPublicKeyInfo_sequence_TLV
+            serialize_subjectPublicKeyInfo
             `serialize_nondep_then`
-            serialize_fwid_sequence_TLV)
-  (* g1 *) (synth_compositeDeviceID_t')
+            serialize_fwid)
+  (* g1 *) (synth_compositeDeviceID_payload_t')
   (* prf*) ()
 
-let lemma_serialize_compositeDeviceID_unfold
-  (x: compositeDeviceID_t)
+let lemma_serialize_compositeDeviceID_payload_unfold
+  (x: compositeDeviceID_payload_t)
 : Lemma (
-  serialize (serialize_compositeDeviceID) x ==
+  serialize (serialize_compositeDeviceID_payload) x ==
   serialize (serialize_asn1_TLV_of_type INTEGER) x.riot_version
   `Seq.append`
-  serialize (serialize_subjectPublicKeyInfo_sequence_TLV) x.riot_deviceID
+  serialize (serialize_subjectPublicKeyInfo) x.riot_deviceID
   `Seq.append`
-  serialize serialize_fwid_sequence_TLV x.riot_fwid
-  // (* unfold subjectPublicKeyInfo *)
-  // serialize (serialize_subjectPublicKeyInfo) x.riot_deviceID ==
-  // serialize (serialize_algorithmIdentifier_sequence_TLV) x.riot_deviceID.subjectPubKey_alg
-  // `Seq.append`
-  // serialize (serialize_asn1_TLV_of_type BIT_STRING) x.riot_deviceID.subjectPubKey /\
-  // (* unfold FWID *)
-  // serialize serialize_fwid x.riot_fwid ==
-  // serialize (serialize_asn1_TLV_of_type OID) x.riot_fwid.fwid_hashAlg
-  // `Seq.append`
-  // serialize (serialize_asn1_TLV_of_type OCTET_STRING) x.riot_fwid.fwid_value
+  serialize serialize_fwid x.riot_fwid
 )
 = serialize_nondep_then_eq
   (* s1 *) (serialize_asn1_TLV_of_type INTEGER)
-  (* s2 *) (serialize_subjectPublicKeyInfo_sequence_TLV)
-  (* in *) (fst (synth_compositeDeviceID_t' x));
+  (* s2 *) (serialize_subjectPublicKeyInfo)
+  (* in *) (fst (synth_compositeDeviceID_payload_t' x));
   serialize_nondep_then_eq
   (* s1 *) (serialize_asn1_TLV_of_type INTEGER
             `serialize_nondep_then`
-            serialize_subjectPublicKeyInfo_sequence_TLV)
-  (* s2 *) (serialize_fwid_sequence_TLV)
-  (* in *) (synth_compositeDeviceID_t' x);
+            serialize_subjectPublicKeyInfo)
+  (* s2 *) (serialize_fwid)
+  (* in *) (synth_compositeDeviceID_payload_t' x);
   serialize_synth_eq
   (* p1 *) (parse_asn1_TLV_of_type INTEGER
             `nondep_then`
-            parse_subjectPublicKeyInfo_sequence_TLV
+            parse_subjectPublicKeyInfo
             `nondep_then`
-            parse_fwid_sequence_TLV)
-  (* f2 *) (synth_compositeDeviceID_t)
+            parse_fwid)
+  (* f2 *) (synth_compositeDeviceID_payload_t)
   (* s1 *) (serialize_asn1_TLV_of_type INTEGER
             `serialize_nondep_then`
-            serialize_subjectPublicKeyInfo_sequence_TLV
+            serialize_subjectPublicKeyInfo
             `serialize_nondep_then`
-            serialize_fwid_sequence_TLV)
-  (* g1 *) (synth_compositeDeviceID_t')
+            serialize_fwid)
+  (* g1 *) (synth_compositeDeviceID_payload_t')
   (* prf*) ()
   (* in *) x
-    // lemma_serialize_subjectPublicKeyInfo_sequence_TLV_unfold   x.riot_deviceID;
-    // lemma_serialize_subjectPublicKeyInfo_unfold                x.riot_deviceID;
-    //   lemma_serialize_algorithmIdentifier_sequence_TLV_unfold x.riot_deviceID.subjectPubKey_alg;
-    //   lemma_serialize_algorithmIdentifier_sequence_TLV_size   x.riot_deviceID.subjectPubKey_alg;
-    // lemma_serialize_fwid_sequence_TLV_unfold x.riot_fwid;
-    // lemma_serialize_fwid_unfold              x.riot_fwid
 
 #set-options "--z3rlimit 32 --fuel 0 --ifuel 0"
-let lemma_serialize_compositeDeviceID_size
-  (x: compositeDeviceID_t)
+let lemma_serialize_compositeDeviceID_payload_size
+  (x: compositeDeviceID_payload_t)
 : Lemma (
-  length_of_opaque_serialization (serialize_compositeDeviceID) x ==
+  length_of_opaque_serialization (serialize_compositeDeviceID_payload) x ==
   length_of_asn1_primitive_TLV x.riot_version +
-  length_of_opaque_serialization (serialize_subjectPublicKeyInfo_sequence_TLV) x.riot_deviceID +
-  length_of_opaque_serialization serialize_fwid_sequence_TLV x.riot_fwid /\
-  length_of_opaque_serialization serialize_compositeDeviceID x ==
+  length_of_opaque_serialization (serialize_subjectPublicKeyInfo) x.riot_deviceID +
+  length_of_opaque_serialization serialize_fwid x.riot_fwid /\
+  length_of_opaque_serialization serialize_compositeDeviceID_payload x ==
   length_of_asn1_primitive_TLV x.riot_version + 91 /\
-  length_of_opaque_serialization serialize_compositeDeviceID x <= 97
+  length_of_opaque_serialization serialize_compositeDeviceID_payload x <= 97
 )
-= lemma_serialize_compositeDeviceID_unfold x;
-    lemma_serialize_subjectPublicKeyInfo_sequence_TLV_size_exact x.riot_deviceID;
-    lemma_serialize_fwid_sequence_TLV_size_exact x.riot_fwid
+= lemma_serialize_compositeDeviceID_payload_unfold x;
+    lemma_serialize_subjectPublicKeyInfo_size_exact x.riot_deviceID;
+    lemma_serialize_fwid_size_exact x.riot_fwid
 
 (* inbound sub type*)
 // unfold
-let compositeDeviceID_t_inbound
-= inbound_sequence_value_of (serialize_compositeDeviceID)
+let compositeDeviceID_t
+= inbound_sequence_value_of (serialize_compositeDeviceID_payload)
 
 (* TLV serializer *)
-let parse_compositeDeviceID_sequence_TLV
-: parser (parse_asn1_envelop_tag_with_TLV_kind SEQUENCE) (compositeDeviceID_t_inbound)
-= compositeDeviceID_t_inbound
+let parse_compositeDeviceID
+: parser (parse_asn1_envelop_tag_with_TLV_kind SEQUENCE) (compositeDeviceID_t)
+= compositeDeviceID_t
   `coerce_parser`
-  parse_asn1_sequence_TLV (serialize_compositeDeviceID)
+  parse_asn1_sequence_TLV (serialize_compositeDeviceID_payload)
 
-let serialize_compositeDeviceID_sequence_TLV
-: serializer (parse_compositeDeviceID_sequence_TLV)
+let serialize_compositeDeviceID
+: serializer (parse_compositeDeviceID)
 = coerce_parser_serializer
-  (* t *) (parse_compositeDeviceID_sequence_TLV)
-  (* s *) (serialize_asn1_sequence_TLV (serialize_compositeDeviceID))
+  (* t *) (parse_compositeDeviceID)
+  (* s *) (serialize_asn1_sequence_TLV (serialize_compositeDeviceID_payload))
   (*prf*) ()
 
 (* manually unfolding `lemma_serialize_asn1_sequence_TLV_size` to avoid stuck here.  *)
-let lemma_serialize_compositeDeviceID_sequence_TLV_unfold
-  (x: compositeDeviceID_t_inbound)
-: Lemma ( predicate_serialize_asn1_sequence_TLV_unfold serialize_compositeDeviceID x )
-= lemma_serialize_asn1_sequence_TLV_unfold serialize_compositeDeviceID x
+let lemma_serialize_compositeDeviceID_unfold
+  (x: compositeDeviceID_t)
+: Lemma ( predicate_serialize_asn1_sequence_TLV_unfold serialize_compositeDeviceID_payload x )
+= lemma_serialize_asn1_sequence_TLV_unfold serialize_compositeDeviceID_payload x
 
-let lemma_serialize_compositeDeviceID_sequence_TLV_size
-  (x: compositeDeviceID_t_inbound)
-: Lemma ( predicate_serialize_asn1_sequence_TLV_size serialize_compositeDeviceID x )
-= lemma_serialize_asn1_sequence_TLV_size serialize_compositeDeviceID x
+let lemma_serialize_compositeDeviceID_size
+  (x: compositeDeviceID_t)
+: Lemma ( predicate_serialize_asn1_sequence_TLV_size serialize_compositeDeviceID_payload x )
+= lemma_serialize_asn1_sequence_TLV_size serialize_compositeDeviceID_payload x
 
 open FStar.Integers
-#push-options "--z3rlimit 32 --fuel 0 --ifuel 0"
-let lemma_serialize_compositeDeviceID_sequence_TLV_size_exact
-  (x: compositeDeviceID_t_inbound)
+#push-options "--z3rlimit 64"
+let lemma_serialize_compositeDeviceID_size_exact
+  (x: compositeDeviceID_t)
 : Lemma (
-  length_of_opaque_serialization serialize_compositeDeviceID_sequence_TLV x ==
+  length_of_opaque_serialization serialize_compositeDeviceID x ==
   length_of_asn1_primitive_TLV x.riot_version + 93 /\
-  length_of_opaque_serialization serialize_compositeDeviceID_sequence_TLV x <= 99
+  length_of_opaque_serialization serialize_compositeDeviceID_payload x <= 99
 )
-= lemma_serialize_compositeDeviceID_sequence_TLV_unfold x;
-  lemma_serialize_compositeDeviceID_sequence_TLV_size   x;
-    lemma_serialize_compositeDeviceID_size x;
-    assert (length_of_opaque_serialization serialize_compositeDeviceID_sequence_TLV x ==
-            1 +
-            length_of_asn1_length (u (length_of_opaque_serialization serialize_compositeDeviceID x)) +
-            length_of_opaque_serialization serialize_compositeDeviceID x)
+= lemma_serialize_compositeDeviceID_unfold x;
+  lemma_serialize_compositeDeviceID_size   x;
+    lemma_serialize_compositeDeviceID_payload_size x
 #pop-options
 
-let serialize32_compositeDeviceID_backwards
-: serializer32_backwards (serialize_compositeDeviceID)
+let serialize32_compositeDeviceID_payload_backwards
+: serializer32_backwards (serialize_compositeDeviceID_payload)
 = serialize32_synth_backwards
   (* ls *) (serialize32_asn1_TLV_backwards_of_type INTEGER
             `serialize32_nondep_then_backwards`
-            serialize32_subjectPublicKeyInfo_sequence_TLV_backwards
+            serialize32_subjectPublicKeyInfo_backwards
             `serialize32_nondep_then_backwards`
-            serialize32_fwid_sequence_TLV_backwards)
-  (* f2 *) (synth_compositeDeviceID_t)
-  (* g1 *) (synth_compositeDeviceID_t')
-  (* g1'*) (synth_compositeDeviceID_t')
+            serialize32_fwid_backwards)
+  (* f2 *) (synth_compositeDeviceID_payload_t)
+  (* g1 *) (synth_compositeDeviceID_payload_t')
+  (* g1'*) (synth_compositeDeviceID_payload_t')
   (* prf*) ()
 
-let serialize32_compositeDeviceID_sequence_TLV_backwards
-: serializer32_backwards (serialize_compositeDeviceID_sequence_TLV)
+let serialize32_compositeDeviceID_backwards
+: serializer32_backwards (serialize_compositeDeviceID)
 = coerce_serializer32_backwards
-  (* s2  *) (serialize_compositeDeviceID_sequence_TLV)
+  (* s2  *) (serialize_compositeDeviceID)
   (* s32 *) (serialize32_asn1_sequence_TLV_backwards
-             (* ls *) (serialize32_compositeDeviceID_backwards))
+             (* ls *) (serialize32_compositeDeviceID_payload_backwards))
   (* prf *) ()
 
 (* helpers *)
@@ -210,19 +190,19 @@ let x509_get_compositeDeviceID
   (version: datatype_of_asn1_type INTEGER)
   (deviceKeyPub: B32.lbytes32 32ul)
   (fwid: B32.lbytes32 32ul)
-: Tot (compositeDeviceID_t_inbound)
-= let deviceIDPublicKeyInfo: subjectPublicKeyInfo_t_inbound = x509_get_subjectPublicKeyInfo deviceKeyPub in
-  (* Prf *) lemma_serialize_subjectPublicKeyInfo_sequence_TLV_size_exact deviceIDPublicKeyInfo;
+: Tot (compositeDeviceID_t)
+= let deviceIDPublicKeyInfo: subjectPublicKeyInfo_t = x509_get_subjectPublicKeyInfo deviceKeyPub in
+  (* Prf *) lemma_serialize_subjectPublicKeyInfo_size_exact deviceIDPublicKeyInfo;
 
-  let fwid: fwid_t_inbound = x509_get_fwid fwid in
-  (* Prf *) lemma_serialize_fwid_sequence_TLV_size_exact fwid;
+  let fwid: fwid_payload_t = x509_get_fwid fwid in
+  (* Prf *) lemma_serialize_fwid_size_exact fwid;
 
-  let compositeDeviceID: compositeDeviceID_t = {
+  let compositeDeviceID: compositeDeviceID_payload_t = {
     riot_version  = version;
     riot_deviceID = deviceIDPublicKeyInfo;
     riot_fwid     = fwid
   } in
-  (* Prf *) lemma_serialize_compositeDeviceID_size compositeDeviceID;
+  (* Prf *) lemma_serialize_compositeDeviceID_payload_size compositeDeviceID;
   (* Prf *) (**) lemma_serialize_asn1_integer_TLV_size compositeDeviceID.riot_version;
 
 (* return *) compositeDeviceID
