src/riot/RIoT.X509.Extension.fst
@@ -7,114 +7,111 @@ include RIoT.X509.CompositeDeviceID
 
 open FStar.Integers
 
-(* FIXME: Can not extract this type, disabling them for now *)
-
-let x509_extValue_riot_t = OCTET_STRING
-                           `inbound_envelop_tag_with_value_of`
-                           serialize_compositeDeviceID_sequence_TLV
-
-type riot_extension_t: Type
+#set-options "--z3rlimit 32 --fuel 0 --ifuel 0"
+type riot_extension_payload_t: Type
 = { x509_extID_riot      : x:datatype_of_asn1_type OID {x == OID_RIOT};
     x509_extCritical_riot: datatype_of_asn1_type BOOLEAN;
-    x509_extValue_riot   : x509_extValue_riot_t }
+    x509_extValue_riot   : OCTET_STRING `inbound_envelop_tag_with_value_of`
+                           (**) serialize_compositeDeviceID }
 
-// #pop-options
-
-let synth_riot_extension_t
-  (x': x509_extension_t' OID_RIOT serialize_compositeDeviceID_sequence_TLV)
-: GTot (riot_extension_t)
+let synth_riot_extension_payload_t
+  (x': x509_extension_t' OID_RIOT serialize_compositeDeviceID)
+: GTot (riot_extension_payload_t)
 = { x509_extID_riot       = fst (fst x');
     x509_extCritical_riot = snd (fst x');
     x509_extValue_riot    = snd x' }
 
-let synth_riot_extension_t_inverse
-  (x: riot_extension_t)
-: Tot (x': x509_extension_t' OID_RIOT serialize_compositeDeviceID_sequence_TLV
-           { x == synth_riot_extension_t x' })
+let synth_riot_extension_payload_t_inverse
+  (x: riot_extension_payload_t)
+: Tot (x': x509_extension_t' OID_RIOT serialize_compositeDeviceID
+           { x == synth_riot_extension_payload_t x' })
 = ((x.x509_extID_riot,
     x.x509_extCritical_riot),
     x.x509_extValue_riot)
 
-unfold
-let parse_riot_extension
-: parser parse_x509_extension_kind riot_extension_t
+#set-options "--ifuel 1"
+let parse_riot_extension_payload
+: parser parse_x509_extension_kind riot_extension_payload_t
 = parse_x509_extension
     OID_RIOT
-    serialize_compositeDeviceID_sequence_TLV
-    synth_riot_extension_t
+    serialize_compositeDeviceID
+    synth_riot_extension_payload_t
     ()
 
-unfold
-let serialize_riot_extension
-: serializer parse_riot_extension
+let serialize_riot_extension_payload
+: serializer parse_riot_extension_payload
 = serialize_x509_extension
     OID_RIOT
-    serialize_compositeDeviceID_sequence_TLV
-    synth_riot_extension_t
-    synth_riot_extension_t_inverse
+    serialize_compositeDeviceID
+    synth_riot_extension_payload_t
+    synth_riot_extension_payload_t_inverse
     ()
 
-let lemma_serialize_riot_extension_unfold
+let lemma_serialize_riot_extension_payload_unfold
 = lemma_serialize_x509_extension_unfold
     OID_RIOT
-    serialize_compositeDeviceID_sequence_TLV
-    synth_riot_extension_t
-    synth_riot_extension_t_inverse
+    serialize_compositeDeviceID
+    synth_riot_extension_payload_t
+    synth_riot_extension_payload_t_inverse
     ()
 
-let lemma_serialize_riot_extension_size
+let lemma_serialize_riot_extension_payload_size
 = lemma_serialize_x509_extension_size
     OID_RIOT
-    serialize_compositeDeviceID_sequence_TLV
-    synth_riot_extension_t
-    synth_riot_extension_t_inverse
+    serialize_compositeDeviceID
+    synth_riot_extension_payload_t
+    synth_riot_extension_payload_t_inverse
     ()
 
-let riot_extension_t_inbound
+(*
+ *
+ *)
+
+let riot_extension_t
 = x509_extension_t_inbound
     OID_RIOT
-    serialize_compositeDeviceID_sequence_TLV
-    synth_riot_extension_t
-    synth_riot_extension_t_inverse
+    serialize_compositeDeviceID
+    synth_riot_extension_payload_t
+    synth_riot_extension_payload_t_inverse
     ()
 
-let parse_riot_extension_sequence_TLV
-: parser parse_x509_extension_sequence_TLV_kind riot_extension_t_inbound
-= riot_extension_t_inbound
+let parse_riot_extension
+: parser parse_x509_extension_sequence_TLV_kind riot_extension_t
+= riot_extension_t
   `coerce_parser`
   parse_x509_extension_sequence_TLV
     OID_RIOT
-    serialize_compositeDeviceID_sequence_TLV
-    synth_riot_extension_t
-    synth_riot_extension_t_inverse
+    serialize_compositeDeviceID
+    synth_riot_extension_payload_t
+    synth_riot_extension_payload_t_inverse
     ()
 
-let serialize_riot_extension_sequence_TLV
-: serializer parse_riot_extension_sequence_TLV
+let serialize_riot_extension
+: serializer parse_riot_extension
 = coerce_parser_serializer
-  (* p2 *) parse_riot_extension_sequence_TLV
+  (* p2 *) parse_riot_extension
   (* s1 *) (serialize_x509_extension_sequence_TLV
               OID_RIOT
-              serialize_compositeDeviceID_sequence_TLV
-              synth_riot_extension_t
-              synth_riot_extension_t_inverse
+              serialize_compositeDeviceID
+              synth_riot_extension_payload_t
+              synth_riot_extension_payload_t_inverse
               ())
   (* prf*) ()
 
-let lemma_serialize_riot_extension_sequence_TLV_unfold
+let lemma_serialize_riot_extension_unfold
 = lemma_serialize_x509_extension_sequence_TLV_unfold
     OID_RIOT
-    serialize_compositeDeviceID_sequence_TLV
-    synth_riot_extension_t
-    synth_riot_extension_t_inverse
+    serialize_compositeDeviceID
+    synth_riot_extension_payload_t
+    synth_riot_extension_payload_t_inverse
     ()
 
-let lemma_serialize_riot_extension_sequence_TLV_size
+let lemma_serialize_riot_extension_size
 = lemma_serialize_x509_extension_sequence_TLV_size
     OID_RIOT
-    serialize_compositeDeviceID_sequence_TLV
-    synth_riot_extension_t
-    synth_riot_extension_t_inverse
+    serialize_compositeDeviceID
+    synth_riot_extension_payload_t
+    synth_riot_extension_payload_t_inverse
     ()
 
 let length_of_riot_extension_payload
@@ -130,17 +127,17 @@ let len_of_riot_extension_payload
 = len_of_asn1_primitive_TLV version + 109ul
 
 #push-options "--z3rlimit 128 --fuel 0 --ifuel 2"
-let lemma_serialize_riot_extension_size_exact
-  (x: riot_extension_t_inbound)
+let lemma_serialize_riot_extension_payload_size_exact
+  (x: riot_extension_t)
 : Lemma (
-  length_of_opaque_serialization serialize_riot_extension x ==
+  length_of_opaque_serialization serialize_riot_extension_payload x ==
   length_of_riot_extension_payload x.x509_extValue_riot.riot_version /\
-  length_of_opaque_serialization serialize_riot_extension x <= 115
+  length_of_opaque_serialization serialize_riot_extension_payload x <= 115
 )
-= lemma_serialize_riot_extension_size x;
+= lemma_serialize_riot_extension_payload_size x;
   assert (length_of_asn1_primitive_TLV x.x509_extID_riot == 11);
-  lemma_serialize_compositeDeviceID_sequence_TLV_size_exact x.x509_extValue_riot;
-  assert (length_of_TLV OCTET_STRING (length_of_opaque_serialization serialize_compositeDeviceID_sequence_TLV x.x509_extValue_riot)
+  lemma_serialize_compositeDeviceID_size_exact x.x509_extValue_riot;
+  assert (length_of_TLV OCTET_STRING (length_of_opaque_serialization serialize_compositeDeviceID x.x509_extValue_riot)
           == length_of_asn1_primitive_TLV x.x509_extValue_riot.riot_version + 95)
 
 let length_of_riot_extension
@@ -155,42 +152,42 @@ let len_of_riot_extension
             { v len == length_of_riot_extension version })
 = len_of_TLV SEQUENCE (len_of_riot_extension_payload version)
 
-let lemma_serialize_riot_extension_sequence_TLV_size_exact
-  (x: riot_extension_t_inbound)
+let lemma_serialize_riot_extension_size_exact
+  (x: riot_extension_t)
 : Lemma (
-  length_of_opaque_serialization serialize_riot_extension_sequence_TLV x ==
+  length_of_opaque_serialization serialize_riot_extension x ==
   length_of_riot_extension x.x509_extValue_riot.riot_version /\
-  length_of_opaque_serialization serialize_riot_extension_sequence_TLV x <= 117
+  length_of_opaque_serialization serialize_riot_extension x <= 117
 )
-= lemma_serialize_riot_extension_sequence_TLV_size x;
-  lemma_serialize_riot_extension_size_exact x
+= lemma_serialize_riot_extension_size x;
+  lemma_serialize_riot_extension_payload_size_exact x
 #pop-options
 
 (* low *)
 open ASN1.Low
 
-let serialize32_riot_extension_backwards
-: serializer32_backwards serialize_riot_extension
+let serialize32_riot_extension_payload_backwards
+: serializer32_backwards serialize_riot_extension_payload
 = coerce_serializer32_backwards
-  (* s2 *) (serialize_riot_extension)
+  (* s2 *) (serialize_riot_extension_payload)
   (* s32*) (serialize32_x509_extension_backwards
               OID_RIOT
-              serialize32_compositeDeviceID_sequence_TLV_backwards
-              synth_riot_extension_t
-              synth_riot_extension_t_inverse
-              synth_riot_extension_t_inverse
+              serialize32_compositeDeviceID_backwards
+              synth_riot_extension_payload_t
+              synth_riot_extension_payload_t_inverse
+              synth_riot_extension_payload_t_inverse
               ())
   (* prf*) ()
 
-let serialize32_riot_extension_sequence_TLV_backwards
+let serialize32_riot_extension_backwards
 = coerce_serializer32_backwards
-  (* s2 *) (serialize_riot_extension_sequence_TLV)
+  (* s2 *) (serialize_riot_extension)
   (* s32*) (serialize32_x509_extension_sequence_TLV_backwards
               OID_RIOT
-              serialize32_compositeDeviceID_sequence_TLV_backwards
-              synth_riot_extension_t
-              synth_riot_extension_t_inverse
-              synth_riot_extension_t_inverse
+              serialize32_compositeDeviceID_backwards
+              synth_riot_extension_payload_t
+              synth_riot_extension_payload_t_inverse
+              synth_riot_extension_payload_t_inverse
               ())
   (* prf*) ()
 
@@ -203,18 +200,18 @@ let x509_get_riot_extension
   (version: datatype_of_asn1_type INTEGER)
   (fwid: B32.lbytes32 32ul)
   (deviceIDPub: B32.lbytes32 32ul)
-: Tot (riot_extension_t_inbound)
+: Tot (riot_extension_t)
 =
-  let compositeDeviceID: compositeDeviceID_t_inbound = x509_get_compositeDeviceID version deviceIDPub fwid in
-  (* Prf *) lemma_serialize_compositeDeviceID_sequence_TLV_size_exact compositeDeviceID;
+  let compositeDeviceID: compositeDeviceID_t = x509_get_compositeDeviceID version deviceIDPub fwid in
+  (* Prf *) lemma_serialize_compositeDeviceID_size_exact compositeDeviceID;
 
-  let riot_extension: riot_extension_t = {
+  let riot_extension: riot_extension_payload_t = {
     x509_extID_riot       = OID_RIOT;
     x509_extCritical_riot = false;
     x509_extValue_riot    = compositeDeviceID
   } in
-  (* Prf *) lemma_serialize_riot_extension_unfold riot_extension;
-  (* Prf *) lemma_serialize_riot_extension_size   riot_extension;
+  (* Prf *) lemma_serialize_riot_extension_payload_unfold riot_extension;
+  (* Prf *) lemma_serialize_riot_extension_payload_size   riot_extension;
   (* Prf *) (**) lemma_serialize_asn1_oid_TLV_size riot_extension.x509_extID_riot;
   (* Prf *) (**) lemma_serialize_asn1_boolean_TLV_size riot_extension.x509_extCritical_riot;
 
