src/riot/RIoT.X509.FWID.fst
@@ -15,62 +15,62 @@ open FStar.Integers
 (* FWID
   ======
 *)
-type fwid_t = {
+type fwid_payload_t = {
   fwid_hashAlg: x:datatype_of_asn1_type OID {x == OID_DIGEST_SHA256}; (* OID *)
   fwid_value  : x:datatype_of_asn1_type OCTET_STRING {v (dfst x) == 32}
 }
 
-let filter_fwid
+let filter_fwid_payload
   (x': datatype_of_asn1_type OID `tuple2` datatype_of_asn1_type OCTET_STRING)
 : GTot bool
 = fst x' = OID_DIGEST_SHA256 &&
   v (dfst (snd x')) = 32
 
-let fwid_t' = parse_filter_refine filter_fwid
+let fwid_payload_t' = parse_filter_refine filter_fwid_payload
 
 (* Serialier spec *)
-let synth_fwid_t
-  (x': fwid_t')
-: GTot (fwid_t)
+let synth_fwid_payload_t
+  (x': fwid_payload_t')
+: GTot (fwid_payload_t)
 = { fwid_hashAlg = fst x';
     fwid_value   = snd x' }
 
-let synth_fwid_t'
-  (x: fwid_t)
-: Tot (x': fwid_t' { x == synth_fwid_t x' } )
+let synth_fwid_payload_t'
+  (x: fwid_payload_t)
+: Tot (x': fwid_payload_t' { x == synth_fwid_payload_t x' } )
 = (x.fwid_hashAlg, x.fwid_value)
 
-let parse_fwid
-: parser _ fwid_t
+let parse_fwid_payload
+: parser _ fwid_payload_t
 = parse_asn1_TLV_of_type OID
   `nondep_then`
   parse_asn1_TLV_of_type OCTET_STRING
   `parse_filter`
-  filter_fwid
+  filter_fwid_payload
   `parse_synth`
-  synth_fwid_t
+  synth_fwid_payload_t
 
-let serialize_fwid
-: serializer parse_fwid
+let serialize_fwid_payload
+: serializer parse_fwid_payload
 = serialize_synth
   (* p1 *) (parse_asn1_TLV_of_type OID
             `nondep_then`
             parse_asn1_TLV_of_type OCTET_STRING
             `parse_filter`
-            filter_fwid)
-  (* f2 *) (synth_fwid_t)
+            filter_fwid_payload)
+  (* f2 *) (synth_fwid_payload_t)
   (* s1 *) (serialize_asn1_TLV_of_type OID
             `serialize_nondep_then`
             serialize_asn1_TLV_of_type OCTET_STRING
             `serialize_filter`
-            filter_fwid)
-  (* g1 *) (synth_fwid_t')
+            filter_fwid_payload)
+  (* g1 *) (synth_fwid_payload_t')
   (* prf*) ()
 
-let lemma_serialize_fwid_unfold
-  (x: fwid_t)
+let lemma_serialize_fwid_payload_unfold
+  (x: fwid_payload_t)
 : Lemma (
-  serialize serialize_fwid x ==
+  serialize serialize_fwid_payload x ==
   serialize serialize_asn1_oid_TLV x.fwid_hashAlg
   `Seq.append`
   serialize serialize_asn1_octet_string_TLV x.fwid_value
@@ -78,92 +78,100 @@ let lemma_serialize_fwid_unfold
 = serialize_nondep_then_eq
   (* s1 *) (serialize_asn1_TLV_of_type OID)
   (* s2 *) (serialize_asn1_TLV_of_type OCTET_STRING)
-  (* in *) (synth_fwid_t' x);
+  (* in *) (synth_fwid_payload_t' x);
   serialize_synth_eq
   (* p1 *) (parse_asn1_TLV_of_type OID
             `nondep_then`
             parse_asn1_TLV_of_type OCTET_STRING
             `parse_filter`
-            filter_fwid)
-  (* f2 *) (synth_fwid_t)
+            filter_fwid_payload)
+  (* f2 *) (synth_fwid_payload_t)
   (* s1 *) (serialize_asn1_TLV_of_type OID
             `serialize_nondep_then`
             serialize_asn1_TLV_of_type OCTET_STRING
             `serialize_filter`
-            filter_fwid)
-  (* g1 *) (synth_fwid_t')
+            filter_fwid_payload)
+  (* g1 *) (synth_fwid_payload_t')
   (* prf*) ()
   (* in *) x
 
 #push-options "--z3rlimit 32"
-let lemma_serialize_fwid_size
-  (x: fwid_t)
+let lemma_serialize_fwid_payload_size
+  (x: fwid_payload_t)
 : Lemma (
-  Seq.length (serialize serialize_fwid x) ==
+  Seq.length (serialize serialize_fwid_payload x) ==
   length_of_asn1_primitive_TLV x.fwid_hashAlg +
   length_of_asn1_primitive_TLV x.fwid_value /\
-  Seq.length (serialize serialize_fwid x) == 45
+  Seq.length (serialize serialize_fwid_payload x) == 45
 )
-= lemma_serialize_fwid_unfold x;
+= lemma_serialize_fwid_payload_unfold x;
   assert_norm (length_of_asn1_primitive_TLV x.fwid_hashAlg == 11);
   assert_norm (length_of_asn1_primitive_TLV x.fwid_value == 34)
 #pop-options
 
 (* inbound sub type*)
-let fwid_t_inbound
-= inbound_sequence_value_of serialize_fwid
+let fwid_t
+= inbound_sequence_value_of serialize_fwid_payload
 
 (* TLV serializer *)
-let parse_fwid_sequence_TLV
-: parser _ fwid_t_inbound
-= parse_asn1_sequence_TLV serialize_fwid
+let parse_fwid
+: parser (parse_asn1_envelop_tag_with_TLV_kind SEQUENCE) fwid_t
+= fwid_t
+  `coerce_parser`
+  parse_asn1_sequence_TLV serialize_fwid_payload
 
-let serialize_fwid_sequence_TLV
-: serializer parse_fwid_sequence_TLV
-= serialize_asn1_sequence_TLV serialize_fwid
+let serialize_fwid
+: serializer parse_fwid
+= coerce_parser_serializer
+  (* p *) (parse_fwid)
+  (* s *) (serialize_asn1_sequence_TLV serialize_fwid_payload)
+  (*prf*) ()
 
-let lemma_serialize_fwid_sequence_TLV_unfold
-  (x: fwid_t_inbound)
-: Lemma ( predicate_serialize_asn1_sequence_TLV_unfold serialize_fwid x )
-= lemma_serialize_asn1_sequence_TLV_unfold serialize_fwid x
+let lemma_serialize_fwid_unfold
+  (x: fwid_t)
+: Lemma ( predicate_serialize_asn1_sequence_TLV_unfold serialize_fwid_payload x )
+= lemma_serialize_asn1_sequence_TLV_unfold serialize_fwid_payload x
 
-let lemma_serialize_fwid_sequence_TLV_size
-  (x: fwid_t_inbound)
-: Lemma ( predicate_serialize_asn1_sequence_TLV_size serialize_fwid x )
-= lemma_serialize_asn1_sequence_TLV_size serialize_fwid x
+let lemma_serialize_fwid_size
+  (x: fwid_t)
+: Lemma ( predicate_serialize_asn1_sequence_TLV_size serialize_fwid_payload x )
+= lemma_serialize_asn1_sequence_TLV_size serialize_fwid_payload x
 
 /// 1 + 1 + 45
 #restart-solver
 #push-options "--z3rlimit 32 --fuel 4 --ifuel 4"
-let lemma_serialize_fwid_sequence_TLV_size_exact
-  (x: fwid_t_inbound)
+let lemma_serialize_fwid_size_exact
+  (x: fwid_t)
 : Lemma (
-  length_of_opaque_serialization serialize_fwid_sequence_TLV x == 47
+  length_of_opaque_serialization serialize_fwid x == 47
 )
 =
-  lemma_serialize_fwid_sequence_TLV_unfold x;
-  lemma_serialize_fwid_sequence_TLV_size x;
-  lemma_serialize_fwid_size x
+  lemma_serialize_fwid_unfold x;
+  lemma_serialize_fwid_size x;
+  lemma_serialize_fwid_payload_size x
 #pop-options
 
 (* Low *)
-let serialize32_fwid_backwards
-: serializer32_backwards serialize_fwid
+let serialize32_fwid_payload_backwards
+: serializer32_backwards serialize_fwid_payload
 = serialize32_synth_backwards
   (* ls *) (serialize32_asn1_TLV_backwards_of_type OID
             `serialize32_nondep_then_backwards`
             serialize32_asn1_TLV_backwards_of_type OCTET_STRING
             `serialize32_filter_backwards`
-            filter_fwid)
-  (* f2 *) (synth_fwid_t)
-  (* g1 *) (synth_fwid_t')
-  (* g1'*) (synth_fwid_t')
+            filter_fwid_payload)
+  (* f2 *) (synth_fwid_payload_t)
+  (* g1 *) (synth_fwid_payload_t')
+  (* g1'*) (synth_fwid_payload_t')
   (* prf*) ()
 
-let serialize32_fwid_sequence_TLV_backwards
-: serializer32_backwards serialize_fwid_sequence_TLV
-= serialize32_asn1_sequence_TLV_backwards
-  (* ls *) (serialize32_fwid_backwards)
+let serialize32_fwid_backwards
+: serializer32_backwards serialize_fwid
+= coerce_serializer32_backwards
+  (* s  *) (serialize_fwid)
+  (* s32*) (serialize32_asn1_sequence_TLV_backwards
+           (* ls *) (serialize32_fwid_payload_backwards))
+  (* prf*) ()
 
 module B32 = FStar.Bytes
 
@@ -171,13 +179,13 @@ module B32 = FStar.Bytes
 #push-options "--z3rlimit 8 --fuel 0 --ifuel 0"
 let x509_get_fwid
   (fwid: B32.lbytes32 32ul)
-: Tot (fwid_t_inbound)
+: Tot (fwid_t)
 =
-  let fwid: fwid_t = {
+  let fwid: fwid_payload_t = {
     fwid_hashAlg = OID_DIGEST_SHA256;
     fwid_value   = (|32ul, fwid|)
   } in
-  (* Prf *) lemma_serialize_fwid_size fwid;
+  (* Prf *) lemma_serialize_fwid_payload_size fwid;
   (* Prf *) (**) lemma_serialize_asn1_oid_TLV_size fwid.fwid_hashAlg;
   (* Prf *) (**) lemma_serialize_asn1_octet_string_TLV_size fwid.fwid_value;
 
