src/riot/x509/X509.Crypto.AlgorithmIdentifier.fst
@@ -27,15 +27,14 @@ type algorithmIdentifier_Ed25519_t = {
   algID_ed25519: oid: datatype_of_asn1_type OID { oid == OID_ED25519 }
 }
 
-let algorithmIdentifier_t
+let algorithmIdentifier_payload_t
   // (alg: supported_crypto_alg_t)
 = algorithmIdentifier_Ed25519_t
   // match alg with
   // | AlgID_ECDSA_P256 -> algorithmIdentifier_ECDSA_P256_t
   // | AlgID_Ed25519    -> algorithmIdentifier_Ed25519_t
 
-private
-let algorithmIdentifier_t'_aux
+let algorithmIdentifier_payload_t'_aux
   // (alg: supported_crypto_alg_t)
 =
   // match alg with
@@ -44,9 +43,9 @@ let algorithmIdentifier_t'_aux
   datatype_of_asn1_type OID
 
 /// tuple repr
-let filter_algorithmIdentifier_t'
+let filter_algorithmIdentifier_payload_t'
   // (alg: supported_crypto_alg_t)
-  (x': algorithmIdentifier_t'_aux)
+  (x': algorithmIdentifier_payload_t'_aux)
 : GTot bool
 =
   // match alg with
@@ -57,15 +56,15 @@ let filter_algorithmIdentifier_t'
   ( let x' = x'<: datatype_of_asn1_type OID in
                     x' = OID_ED25519 )
 
-let algorithmIdentifier_t'
+let algorithmIdentifier_payload_t'
   // (alg: supported_crypto_alg_t)
-= parse_filter_refine (filter_algorithmIdentifier_t')
+= parse_filter_refine (filter_algorithmIdentifier_payload_t')
 
 /// tuple repr -> record repr
-let synth_algorithmIdentifier_t
+let synth_algorithmIdentifier_payload_t
   // (alg: supported_crypto_alg_t)
-  (x': algorithmIdentifier_t')
-: GTot (algorithmIdentifier_t)
+  (x': algorithmIdentifier_payload_t')
+: GTot (algorithmIdentifier_payload_t)
 =
   // match alg with
   // | AlgID_ECDSA_P256 -> ( let x' = x' <: tuple2 (datatype_of_asn1_type OID) (datatype_of_asn1_type OID) in
@@ -78,10 +77,10 @@ let synth_algorithmIdentifier_t
 /// record repr -> tuple repr
 
 inline_for_extraction noextract
-let synth_algorithmIdentifier_t'
+let synth_algorithmIdentifier_payload_t'
   // (alg: supported_crypto_alg_t)
-  (x: algorithmIdentifier_t)
-: Tot (x': algorithmIdentifier_t' { x == synth_algorithmIdentifier_t x' })
+  (x: algorithmIdentifier_payload_t)
+: Tot (x': algorithmIdentifier_payload_t' { x == synth_algorithmIdentifier_payload_t x' })
 =
   // match alg with
   // | AlgID_ECDSA_P256 -> ( let x = x <: algorithmIdentifier_ECDSA_P256_t in
@@ -91,7 +90,7 @@ let synth_algorithmIdentifier_t'
   ( let x = x<: algorithmIdentifier_Ed25519_t in
                     x.algID_ed25519 )
 
-let parse_algorithmIdentifier_kind
+let parse_algorithmIdentifier_payload_kind
   // (alg: supported_crypto_alg_t)
 : parser_kind
 =
@@ -103,29 +102,29 @@ let parse_algorithmIdentifier_kind
   ( parse_asn1_TLV_kind_of_type OID )
 
 /// sequence value (body) parser
-let parse_algorithmIdentifier
+let parse_algorithmIdentifier_payload
   // (alg: supported_crypto_alg_t)
-: parser (parse_algorithmIdentifier_kind) (algorithmIdentifier_t)
+: parser (parse_algorithmIdentifier_payload_kind) (algorithmIdentifier_payload_t)
 =
   // match alg with
   // | AlgID_ECDSA_P256 -> ( parse_asn1_TLV_of_type OID
   //                   `nondep_then`
   //                   parse_asn1_TLV_of_type OID
   //                   `parse_filter`
-  //                   filter_algorithmIdentifier_t' alg
+  //                   filter_algorithmIdentifier_payload_t' alg
   //                   `parse_synth`
-  //                   synth_algorithmIdentifier_t alg )
+  //                   synth_algorithmIdentifier_payload_t alg )
   // | AlgID_Ed25519    ->
   ( parse_asn1_TLV_of_type OID
                     `parse_filter`
-                    filter_algorithmIdentifier_t'
+                    filter_algorithmIdentifier_payload_t'
                     `parse_synth`
-                    synth_algorithmIdentifier_t)
+                    synth_algorithmIdentifier_payload_t)
 
 /// sequence value serializer
-let serialize_algorithmIdentifier
+let serialize_algorithmIdentifier_payload
   // (alg: supported_crypto_alg_t)
-: serializer (parse_algorithmIdentifier)
+: serializer (parse_algorithmIdentifier_payload)
 =
   // match alg with
   // | AlgID_ECDSA_P256 -> ( serialize_synth
@@ -133,32 +132,32 @@ let serialize_algorithmIdentifier
   //                             `nondep_then`
   //                             parse_asn1_TLV_of_type OID
   //                             `parse_filter`
-  //                             filter_algorithmIdentifier_t' alg)
-  //                   (* f2 *) (synth_algorithmIdentifier_t alg)
+  //                             filter_algorithmIdentifier_payload_t' alg)
+  //                   (* f2 *) (synth_algorithmIdentifier_payload_t alg)
   //                   (* s1 *) (serialize_asn1_TLV_of_type OID
   //                             `serialize_nondep_then`
   //                             serialize_asn1_TLV_of_type OID
   //                             `serialize_filter`
-  //                             filter_algorithmIdentifier_t' alg)
-  //                   (* g1 *) (synth_algorithmIdentifier_t' alg)
+  //                             filter_algorithmIdentifier_payload_t' alg)
+  //                   (* g1 *) (synth_algorithmIdentifier_payload_t' alg)
   //                   (* prf*) () )
 
   // | AlgID_Ed25519    ->
                            ( serialize_synth
                     (* p1 *) (parse_asn1_TLV_of_type OID
                               `parse_filter`
-                              filter_algorithmIdentifier_t')
-                    (* f2 *) (synth_algorithmIdentifier_t)
+                              filter_algorithmIdentifier_payload_t')
+                    (* f2 *) (synth_algorithmIdentifier_payload_t)
                     (* s1 *) (serialize_asn1_TLV_of_type OID
                               `serialize_filter`
-                              filter_algorithmIdentifier_t')
-                    (* g1 *) (synth_algorithmIdentifier_t')
+                              filter_algorithmIdentifier_payload_t')
+                    (* g1 *) (synth_algorithmIdentifier_payload_t')
                     (* prf*) () )
 
 /// lemma: unfold sequence value serializer
-let lemma_serialize_algorithmIdentifier_unfold
+let lemma_serialize_algorithmIdentifier_payload_unfold
   // (alg: supported_crypto_alg_t)
-  (x: algorithmIdentifier_t)
+  (x: algorithmIdentifier_payload_t)
 : Lemma (
   // match alg with
   // | AlgID_ECDSA_P256 -> ( serialize (serialize_algorithmIdentifier alg) x ==
@@ -166,9 +165,9 @@ let lemma_serialize_algorithmIdentifier_unfold
   //                   `Seq.append`
   //                   serialize (serialize_asn1_TLV_of_type OID) OID_EC_GRP_SECP256R1 )
   // | AlgID_Ed25519    ->
-                   ( serialize (serialize_algorithmIdentifier) x ==
+                   ( serialize (serialize_algorithmIdentifier_payload) x ==
                     serialize (serialize_asn1_TLV_of_type OID) OID_ED25519 /\
-                    length_of_opaque_serialization (serialize_algorithmIdentifier) x ==
+                    length_of_opaque_serialization (serialize_algorithmIdentifier_payload) x ==
                     5
                     ))
 =
@@ -176,32 +175,32 @@ let lemma_serialize_algorithmIdentifier_unfold
   // | AlgID_ECDSA_P256 -> ( serialize_nondep_then_eq
   //                   (* s1 *) (serialize_asn1_TLV_of_type OID)
   //                   (* s2 *) (serialize_asn1_TLV_of_type OID)
-  //                   (* in *) (synth_algorithmIdentifier_t' alg x);
+  //                   (* in *) (synth_algorithmIdentifier_payload_t' alg x);
   //                   serialize_synth_eq
   //                   (* p1 *) (parse_asn1_TLV_of_type OID
   //                             `nondep_then`
   //                             parse_asn1_TLV_of_type OID
   //                             `parse_filter`
-  //                             filter_algorithmIdentifier_t' alg)
-  //                   (* f2 *) (synth_algorithmIdentifier_t alg)
+  //                             filter_algorithmIdentifier_payload_t' alg)
+  //                   (* f2 *) (synth_algorithmIdentifier_payload_t alg)
   //                   (* s1 *) (serialize_asn1_TLV_of_type OID
   //                             `serialize_nondep_then`
   //                             serialize_asn1_TLV_of_type OID
   //                             `serialize_filter`
-  //                             filter_algorithmIdentifier_t' alg)
-  //                   (* g1 *) (synth_algorithmIdentifier_t' alg)
+  //                             filter_algorithmIdentifier_payload_t' alg)
+  //                   (* g1 *) (synth_algorithmIdentifier_payload_t' alg)
   //                   (* prf*) ()
   //                   (* in *) x )
   // | AlgID_Ed25519    ->
                           ( serialize_synth_eq
                     (* p1 *) (parse_asn1_TLV_of_type OID
                               `parse_filter`
-                              filter_algorithmIdentifier_t')
-                    (* f2 *) (synth_algorithmIdentifier_t)
+                              filter_algorithmIdentifier_payload_t')
+                    (* f2 *) (synth_algorithmIdentifier_payload_t)
                     (* s1 *) (serialize_asn1_TLV_of_type OID
                               `serialize_filter`
-                              filter_algorithmIdentifier_t')
-                    (* g1 *) (synth_algorithmIdentifier_t')
+                              filter_algorithmIdentifier_payload_t')
+                    (* g1 *) (synth_algorithmIdentifier_payload_t')
                     (* prf*) ()
                     (* in *) x;
                     assert_norm (length_of_asn1_primitive_TLV OID_ED25519 == 5) )
@@ -210,9 +209,18 @@ let lemma_serialize_algorithmIdentifier_unfold
 ///
 /// lemma: reveal sequence serialization size
 
-let lemma_serialize_algorithmIdentifier_size
+let length_of_algorithmIdentifier_payload ()
+: GTot (asn1_value_length_of_type SEQUENCE)
+= 5
+
+let len_of_algorithmIdentifier_payload ()
+: Tot (len: asn1_value_int32_of_type SEQUENCE
+            { v len == length_of_algorithmIdentifier_payload () })
+= 5ul
+
+let lemma_serialize_algorithmIdentifier_payload_size
   // (alg: supported_crypto_alg_t)
-  (x: algorithmIdentifier_t)
+  (x: algorithmIdentifier_payload_t)
 : Lemma (
   // match alg with
   // | AlgID_ECDSA_P256 -> ( let x = x <: algorithmIdentifier_ECDSA_P256_t in
@@ -221,8 +229,8 @@ let lemma_serialize_algorithmIdentifier_size
   //                   length_of_asn1_primitive_TLV x.alg_id_oid_p256 )
   // | AlgID_Ed25519    ->
                    ( let x = x <: algorithmIdentifier_Ed25519_t in
-                    Seq.length (serialize (serialize_algorithmIdentifier) x) ==
-                    5 )
+                     length_of_opaque_serialization (serialize_algorithmIdentifier_payload) x
+                     == length_of_algorithmIdentifier_payload () )
                     //length_of_asn1_primitive_TLV x.algID_ed25519 /\
                     //x.algID_ed25519 == OID_ED25519 )
                     //length_of_asn1_primitive_TLV x.algID_ed25519 == 5)
@@ -231,85 +239,95 @@ let lemma_serialize_algorithmIdentifier_size
   // match alg with
   // | AlgID_ECDSA_P256 -> ( lemma_serialize_algorithmIdentifier_unfold alg x )
   // | AlgID_Ed25519    ->
-                        ( lemma_serialize_algorithmIdentifier_unfold x;
+                        ( lemma_serialize_algorithmIdentifier_payload_unfold x;
                     assert_norm (length_of_asn1_primitive_TLV x.algID_ed25519 == 5 ))
 
 /// inbound record repr
-let algorithmIdentifier_t_inbound
+let algorithmIdentifier_t
   // (alg: supported_crypto_alg_t)
 =
   // match alg with
   // | AlgID_ECDSA_P256 -> inbound_sequence_value_of (serialize_algorithmIdentifier alg)
   // | AlgID_Ed25519    ->
-  inbound_sequence_value_of (serialize_algorithmIdentifier)
+  inbound_sequence_value_of (serialize_algorithmIdentifier_payload)
 
 /// TLV
 // unfold
-let parse_algorithmIdentifier_sequence_TLV
+let parse_algorithmIdentifier
   // (alg: supported_crypto_alg_t)
-: parser (parse_asn1_envelop_tag_with_TLV_kind SEQUENCE) (algorithmIdentifier_t_inbound)
+: parser (parse_asn1_envelop_tag_with_TLV_kind SEQUENCE) (algorithmIdentifier_t)
 =
   // match alg with
-  // | AlgID_ECDSA_P256 -> ( //algorithmIdentifier_t_inbound alg
+  // | AlgID_ECDSA_P256 -> ( //algorithmIdentifier_t alg
   //                   //`coerce_parser`
   //                   parse_asn1_sequence_TLV (serialize_algorithmIdentifier alg) )
-  // | AlgID_Ed25519    -> ( //algorithmIdentifier_t_inbound alg
+  // | AlgID_Ed25519    -> ( //algorithmIdentifier_t alg
                     //`coerce_parser`
-                    parse_asn1_sequence_TLV (serialize_algorithmIdentifier)
+                    parse_asn1_sequence_TLV (serialize_algorithmIdentifier_payload)
 
-let serialize_algorithmIdentifier_sequence_TLV
+let serialize_algorithmIdentifier
   // (alg: supported_crypto_alg_t)
-: serializer (parse_algorithmIdentifier_sequence_TLV)
+: serializer (parse_algorithmIdentifier)
 =
   // match alg with
   // | AlgID_ECDSA_P256 -> ( serialize_asn1_sequence_TLV (serialize_algorithmIdentifier alg) )
   // | AlgID_Ed25519    ->
-  ( serialize_asn1_sequence_TLV (serialize_algorithmIdentifier) )
+  ( serialize_asn1_sequence_TLV (serialize_algorithmIdentifier_payload) )
 
-let lemma_serialize_algorithmIdentifier_sequence_TLV_unfold
+let lemma_serialize_algorithmIdentifier_unfold
   // (alg: supported_crypto_alg_t)
-  (x: algorithmIdentifier_t_inbound)
-: Lemma ( predicate_serialize_asn1_sequence_TLV_unfold (serialize_algorithmIdentifier) x )
-= lemma_serialize_asn1_sequence_TLV_unfold (serialize_algorithmIdentifier) x
+  (x: algorithmIdentifier_t)
+: Lemma ( predicate_serialize_asn1_sequence_TLV_unfold (serialize_algorithmIdentifier_payload) x )
+= lemma_serialize_asn1_sequence_TLV_unfold (serialize_algorithmIdentifier_payload) x
 
-let lemma_serialize_algorithmIdentifier_sequence_TLV_size
+let lemma_serialize_algorithmIdentifier_size
   // (alg: supported_crypto_alg_t)
-  (x: algorithmIdentifier_t_inbound)
-: Lemma ( predicate_serialize_asn1_sequence_TLV_size (serialize_algorithmIdentifier) x )
+  (x: algorithmIdentifier_t)
+: Lemma ( predicate_serialize_asn1_sequence_TLV_size (serialize_algorithmIdentifier_payload) x )
 =
   // match alg with
   // | AlgID_ECDSA_P256 -> ( lemma_serialize_asn1_sequence_TLV_size (serialize_algorithmIdentifier alg) x )
   // | AlgID_Ed25519    ->
-  ( lemma_serialize_asn1_sequence_TLV_size (serialize_algorithmIdentifier) x )
+  ( lemma_serialize_asn1_sequence_TLV_size (serialize_algorithmIdentifier_payload) x )
+
+let length_of_algorithmIdentifier ()
+: GTot (asn1_TLV_length_of_type SEQUENCE)
+= length_of_TLV SEQUENCE (length_of_algorithmIdentifier_payload ())
+
+let len_of_algorithmIdentifier ()
+: Tot (len: asn1_TLV_int32_of_type SEQUENCE
+            { v len == length_of_algorithmIdentifier () })
+= len_of_TLV SEQUENCE (len_of_algorithmIdentifier_payload ())
 
 #push-options "--z3rlimit 32 --fuel 0 --ifuel 0"
-let lemma_serialize_algorithmIdentifier_sequence_TLV_size_exact
+let lemma_serialize_algorithmIdentifier_size_exact
   // (alg: supported_crypto_alg_t {alg == AlgID_Ed25519})
   (x: algorithmIdentifier_t)
 : Lemma (
   // match alg with
-  // | AlgID_ECDSA_P256 -> ( length_of_opaque_serialization (serialize_algorithmIdentifier_sequence_TLV alg) x == 17 )
+  // | AlgID_ECDSA_P256 -> ( length_of_opaque_serialization (serialize_algorithmIdentifier alg) x == 17 )
   // | AlgID_Ed25519    ->
-                   ( lemma_serialize_algorithmIdentifier_size x;
-                    length_of_opaque_serialization (serialize_algorithmIdentifier_sequence_TLV) x == 7 )
+                   ( lemma_serialize_algorithmIdentifier_payload_size x;
+                     length_of_opaque_serialization (serialize_algorithmIdentifier) x
+                     == length_of_algorithmIdentifier () )
 )
 =
   // match alg with
   // | AlgID_Ed25519    ->
-                  ( lemma_serialize_algorithmIdentifier_size x;
-                    lemma_serialize_asn1_sequence_TLV_unfold (serialize_algorithmIdentifier) x;
-                    lemma_serialize_asn1_sequence_TLV_size   (serialize_algorithmIdentifier) x;
+                  ( lemma_serialize_algorithmIdentifier_payload_size x;
+                    lemma_serialize_asn1_sequence_TLV_unfold (serialize_algorithmIdentifier_payload) x;
+                    lemma_serialize_asn1_sequence_TLV_size   (serialize_algorithmIdentifier_payload) x;
                     // lemma_serialize_algorithmIdentifier_size alg x;
-                    assert (length_of_TLV OID (length_of_opaque_serialization (serialize_algorithmIdentifier) x) == 7) )
+                    assert (length_of_TLV OID (length_of_opaque_serialization (serialize_algorithmIdentifier_payload) x) == 7) )
 #pop-options
 
 /// Low
 ///
 
 inline_for_extraction
-let serialize32_algorithmIdentifier_backwards
+let serialize32_algorithmIdentifier_payload_backwards
   // (alg: supported_crypto_alg_t)
-: serializer32_backwards (serialize_algorithmIdentifier)
+: serializer32_backwards (serialize_algorithmIdentifier_payload)
 =
   // match alg with
   // | AlgID_ECDSA_P256 -> ( serialize32_synth_backwards
@@ -326,23 +344,23 @@ let serialize32_algorithmIdentifier_backwards
                        ( serialize32_synth_backwards
                     (* ls *) (serialize32_asn1_TLV_backwards_of_type OID
                               `serialize32_filter_backwards`
-                              filter_algorithmIdentifier_t')
-                    (* f2 *) (synth_algorithmIdentifier_t)
-                    (* g1 *) (synth_algorithmIdentifier_t')
-                    (* g1'*) (synth_algorithmIdentifier_t')
+                              filter_algorithmIdentifier_payload_t')
+                    (* f2 *) (synth_algorithmIdentifier_payload_t)
+                    (* g1 *) (synth_algorithmIdentifier_payload_t')
+                    (* g1'*) (synth_algorithmIdentifier_payload_t')
                     (* prf*) () )
 
 inline_for_extraction
-let serialize32_algorithmIdentifier_sequence_TLV_backwards
+let serialize32_algorithmIdentifier_backwards
   // (alg: supported_crypto_alg_t)
-: serializer32_backwards (serialize_algorithmIdentifier_sequence_TLV)
+: serializer32_backwards (serialize_algorithmIdentifier)
 =
   // match alg with
   // | AlgID_ECDSA_P256 -> ( serialize32_asn1_sequence_TLV_backwards
   //                   (* s32 *) (serialize32_algorithmIdentifier_backwards alg) )
   // | AlgID_Ed25519    ->
                         ( serialize32_asn1_sequence_TLV_backwards
-                    (* s32 *) (serialize32_algorithmIdentifier_backwards) )
+                    (* s32 *) (serialize32_algorithmIdentifier_payload_backwards) )
 
 (* helpers *)
 
@@ -350,12 +368,12 @@ let serialize32_algorithmIdentifier_sequence_TLV_backwards
 noextract inline_for_extraction
 let x509_get_algorithmIdentifier ()
   // (alg: supported_crypto_alg_t {alg == AlgID_Ed25519})
-: Tot (algorithmIdentifier_t_inbound)
+: Tot (algorithmIdentifier_t)
 =
   // match alg with
   // | AlgID_Ed25519 ->
-                   ( let algID: algorithmIdentifier_t = { algID_ed25519 = OID_ED25519 } in
-                 (* Prf *) lemma_serialize_algorithmIdentifier_size algID;
+                   ( let algID: algorithmIdentifier_payload_t = { algID_ed25519 = OID_ED25519 } in
+                 (* Prf *) lemma_serialize_algorithmIdentifier_payload_size algID;
                  (* Prf *) (**) lemma_serialize_asn1_oid_TLV_size algID.algID_ed25519;
                  (* return *) algID )
 #pop-options
