src/riot/asn1/ASN1.Low.TLV.fst
@@ -112,5 +112,6 @@ unfold
 let len_of_TLV
   (a: asn1_tag_t)
   (len: asn1_value_int32_of_type a)
-: Tot (asn1_TLV_int32_of_type a)
+: Tot (out: asn1_TLV_int32_of_type a
+            { v out == length_of_TLV a (v len) })
 = 1ul + len_of_asn1_length len + len
